<?xml version="1.0" encoding="UTF-8"?> <rdf:RDF xmlns:dc="http://purl.org/dc/elements/1.1/" xmlns:dct="http://purl.org/dc/terms/" xmlns:rdf="http://www.w3.org/1999/02/22-rdf-syntax-ns#" xmlns:schema="https://schema.org/" xmlns:skos="http://www.w3.org/2004/02/skos/core#"> <!-- Scheme: MARC21-008: Format of music --> <skos:ConceptScheme rdf:about="https://doi.org/10.6069/uwlswd.06xx-6744"> <dct:type rdf:resource="http://purl.org/dc/dcmitype/Dataset"/> <dct:title>Music: format of music</dct:title> <dct:alternative>MARC21 008/20 values for music expressed using RDF</dct:alternative> <dct:description>Indicates the format of a musical composition (e.g., piano-conductor score).</dct:description> <dct:publisher rdf:resource="http://viaf.org/viaf/139541794"/> <dct:source rdf:resource="https://www.loc.gov/marc/bibliographic/bd008.html"/> <dct:source rdf:resource="http://marc21rdf.info"/> <dct:provenance rdf:resource="https://doi.org/10.6069/uwlswd.2e2b-y833"/> <dct:creator rdf:resource="http://viaf.org/viaf/139541794"/> <dct:contributor rdf:resource="http://viaf.org/viaf/151962300"/> <dc:contributor>Metadata Management Associates</dc:contributor> <dct:issued>2023</dct:issued> <dc:language>en</dc:language> <dct:license rdf:resource="http://creativecommons.org/publicdomain/zero/1.0"/> <schema:version>1-0-0</schema:version> </skos:ConceptScheme> <!-- Concept: accompaniment reduced for keyboard --> <skos:Concept rdf:about="https://doi.org/10.6069/uwlswd.06xx-6744#c"> <skos:inScheme rdf:resource="https://doi.org/10.6069/uwlswd.06xx-6744"/> <skos:prefLabel xml:lang="en">accompaniment reduced for keyboard</skos:prefLabel> <skos:definition xml:lang="en">Score with instrumental accompaniment reduced for keyboard(s).</skos:definition> <skos:notation xml:lang="en">c</skos:notation> <skos:scopeNote xml:lang="en">Not used for chorus scores and vocal scores.</skos:scopeNote> </skos:Concept> <!-- Concept: chorus score --> <skos:Concept rdf:about="https://doi.org/10.6069/uwlswd.06xx-6744#h"> <skos:inScheme rdf:resource="https://doi.org/10.6069/uwlswd.06xx-6744"/> <skos:prefLabel xml:lang="en">chorus score</skos:prefLabel> <skos:definition xml:lang="en">Score of a work for solo voices and chorus showing only the parts for chorus, with the instrumental accompaniment either arranged for keyboard(s) or other chordal instrument(s) or omitted.</skos:definition> <skos:notation xml:lang="en">h</skos:notation> </skos:Concept> <!-- Concept: close score --> <skos:Concept rdf:about="https://doi.org/10.6069/uwlswd.06xx-6744#g"> <skos:inScheme rdf:resource="https://doi.org/10.6069/uwlswd.06xx-6744"/> <skos:prefLabel xml:lang="en">close score</skos:prefLabel> <skos:definition xml:lang="en">Score (e.g., a hymnal) that has separate parts transcribed in condensed form.</skos:definition> <skos:notation xml:lang="en">g</skos:notation> </skos:Concept> <!-- Concept: condensed score --> <skos:Concept rdf:about="https://doi.org/10.6069/uwlswd.06xx-6744#i"> <skos:inScheme rdf:resource="https://doi.org/10.6069/uwlswd.06xx-6744"/> <skos:prefLabel xml:lang="en">condensed score</skos:prefLabel> <skos:definition xml:lang="en">A score in which the number of staves is reduced to two or a few, generally organized by instrumental sections or vocal parts, and often with cues for individual parts.</skos:definition> <skos:scopeNote xml:lang="en">Used for: Reduced score, Short score.</skos:scopeNote> <skos:notation xml:lang="en">i</skos:notation> </skos:Concept> <!-- Concept: condensed score or piano-conductor score --> <skos:Concept rdf:about="https://doi.org/10.6069/uwlswd.06xx-6744#e"> <skos:inScheme rdf:resource="https://doi.org/10.6069/uwlswd.06xx-6744"/> <skos:prefLabel xml:lang="en">condensed score or piano-conductor score</skos:prefLabel> <skos:definition xml:lang="en">Orchestral or band music that has been reduced. It may be part of an ensemble work for a particular instrument, with cues for other instruments. Such a score is used by an individual playing the instrument for which the score was written or for the conductor.</skos:definition> <skos:notation xml:lang="en">e</skos:notation> </skos:Concept> <!-- Concept: full score --> <skos:Concept rdf:about="https://doi.org/10.6069/uwlswd.06xx-6744#a"> <skos:inScheme rdf:resource="https://doi.org/10.6069/uwlswd.06xx-6744"/> <skos:prefLabel xml:lang="en">full score</skos:prefLabel> <skos:definition xml:lang="en">Staff notation representing the sounds of all the parts of an ensemble (instrumental and/or vocal), arranged so that they can be read simultaneously.</skos:definition> <skos:notation xml:lang="en">a</skos:notation> </skos:Concept> <!-- Concept: full score, miniature or study size --> <skos:Concept rdf:about="https://doi.org/10.6069/uwlswd.06xx-6744#b"> <skos:inScheme rdf:resource="https://doi.org/10.6069/uwlswd.06xx-6744"/> <skos:prefLabel xml:lang="en">miniature or study score</skos:prefLabel> <skos:definition xml:lang="en">Score issued in a musical image of small size, usually redueced from a larger original, and not primarily intended for use in performance.</skos:definition> <skos:notation xml:lang="en">b</skos:notation> </skos:Concept> <!-- Concept: multiple score formats --> <skos:Concept rdf:about="https://doi.org/10.6069/uwlswd.06xx-6744#m"> <skos:inScheme rdf:resource="https://doi.org/10.6069/uwlswd.06xx-6744"/> <skos:prefLabel xml:lang="en">multiple score formats</skos:prefLabel> <skos:definition xml:lang="en">Several types of scores are issued together, as is frequently the case with band music.</skos:definition> <skos:notation xml:lang="en">m</skos:notation> </skos:Concept> <!-- Concept: not applicable --> <skos:Concept rdf:about="https://doi.org/10.6069/uwlswd.06xx-6744#n"> <skos:inScheme rdf:resource="https://doi.org/10.6069/uwlswd.06xx-6744"/> <skos:prefLabel xml:lang="en">not applicable</skos:prefLabel> <skos:definition xml:lang="en">Item is a sound recording.</skos:definition> <skos:notation xml:lang="en">n</skos:notation> </skos:Concept> <!-- Concept: piano score Added by dkt --> <skos:Concept rdf:about="https://doi.org/10.6069/uwlswd.06xx-6744#p"> <skos:inScheme rdf:resource="https://doi.org/10.6069/uwlswd.06xx-6744"/> <skos:prefLabel xml:lang="en">piano score</skos:prefLabel> <skos:definition xml:lang="en">A reduction of an instrumental work or a vocal work with instruments to a version for piano.</skos:definition> <skos:scopeNote xml:lang="en">May include the words of a vocal work.</skos:scopeNote> <skos:notation xml:lang="en">p</skos:notation> </skos:Concept> <!-- Concept: other --> <skos:Concept rdf:about="https://doi.org/10.6069/uwlswd.06xx-6744#z"> <skos:inScheme rdf:resource="https://doi.org/10.6069/uwlswd.06xx-6744"/> <skos:prefLabel xml:lang="en">other</skos:prefLabel> <skos:definition xml:lang="en">Format of music other than full score, miniature or study score, accompaniment reduced for keyboard, voice score with accompaniment omitted, condensed score or piano-conductor score, close score, chorus score, condensed score, performer-conductor part, vocal score, score, multiple score formats, piano score, or unknown.</skos:definition> <skos:notation xml:lang="en">z</skos:notation> </skos:Concept> <!-- Concept: performer-conductor part --> <skos:Concept rdf:about="https://doi.org/10.6069/uwlswd.06xx-6744#j"> <skos:inScheme rdf:resource="https://doi.org/10.6069/uwlswd.06xx-6744"/> <skos:prefLabel xml:lang="en">performer-conductor part</skos:prefLabel> <skos:definition xml:lang="en">A performance part for a single instrument in an ensemble, with cues for the other instruments that enable the performer of that part also to conduct.</skos:definition> <skos:notation xml:lang="en">j</skos:notation> </skos:Concept> <!-- Concept: vocal score Added by dkt --> <skos:Concept rdf:about="https://doi.org/10.6069/uwlswd.06xx-6744#k"> <skos:inScheme rdf:resource="https://doi.org/10.6069/uwlswd.06xx-6744"/> <skos:prefLabel xml:lang="en">vocal score</skos:prefLabel> <skos:definition xml:lang="en">Score showing all vocal parts, solo and/or choral, with the instrumental accompaniment either arranged for keyboard(s) or other chordal instrument(s) or omitted.</skos:definition> <skos:notation xml:lang="en">k</skos:notation> </skos:Concept> <!-- Concept: score Added by dkt --> <skos:Concept rdf:about="https://doi.org/10.6069/uwlswd.06xx-6744#l"> <skos:inScheme rdf:resource="https://doi.org/10.6069/uwlswd.06xx-6744"/> <skos:prefLabel xml:lang="en">score</skos:prefLabel> <skos:definition xml:lang="en">Graphical, symbolic (e.g., staff), or word-based musical notation representing the sounds of all the parts of an ensemble, or a work for solo performer or electronic media. Do not confuse with Part.</skos:definition> <skos:notation xml:lang="en">l</skos:notation> </skos:Concept> <!-- Concept: unknown --> <skos:Concept rdf:about="https://doi.org/10.6069/uwlswd.06xx-6744#u"> <skos:inScheme rdf:resource="https://doi.org/10.6069/uwlswd.06xx-6744"/> <skos:prefLabel xml:lang="en">unknown</skos:prefLabel> <skos:definition xml:lang="en">Format of the item is unknown.</skos:definition> <skos:notation xml:lang="en">u</skos:notation> </skos:Concept> <!-- Concept: voice score --> <skos:Concept rdf:about="https://doi.org/10.6069/uwlswd.06xx-6744#d"> <skos:inScheme rdf:resource="https://doi.org/10.6069/uwlswd.06xx-6744"/> <skos:prefLabel xml:lang="en">voice score with accompaniment omitted</skos:prefLabel> <skos:definition xml:lang="en">Score for solo and/or choral voice(s) with the accompaniment omitted.</skos:definition> <skos:notation xml:lang="en">d</skos:notation> <skos:scopeNote xml:lang="en">Not used for vocal works originally unaccompanied.</skos:scopeNote> </skos:Concept> </rdf:RDF>