<?xml version="1.0" encoding="utf-8"?>
<rdf:RDF
   xmlns:dc="http://purl.org/dc/elements/1.1/"
   xmlns:dct="http://purl.org/dc/terms/"
   xmlns:rdf="http://www.w3.org/1999/02/22-rdf-syntax-ns#"
   xmlns:schema="https://schema.org/"
   xmlns:skos="http://www.w3.org/2004/02/skos/core#"
>
  <rdf:Description rdf:about="https://doi.org/10.6069/uwlswd.qgc0-9r48">
    <rdf:type rdf:resource="http://www.w3.org/2004/02/skos/core#ConceptScheme"/>
    <dct:type rdf:resource="http://purl.org/dc/dcmitype/Dataset"/>
    <dct:title xml:lang="en">Visual: type of visual material</dct:title>
    <dct:alternative xml:lang="en">MARC21 008/33 values for visual materials expressed using RDF</dct:alternative>
    <dct:description xml:lang="en">Indicates the type of visual material being described.</dct:description>
    <schema:disambiguatingDescription xml:lang="en">SKOS Concept Scheme for MARC 00X Values</schema:disambiguatingDescription>
    <dct:publisher rdf:resource="http://viaf.org/viaf/139541794"/>
    <dct:source rdf:resource="https://www.loc.gov/marc/bibliographic/bd008.html"/>
    <dct:source rdf:resource="http://marc21rdf.info"/>
    <dct:provenance rdf:resource="https://doi.org/10.6069/uwlswd.2e2b-y833#marc00Xvalues"/>
    <dct:creator rdf:resource="http://viaf.org/viaf/139541794"/>
    <dct:contributor rdf:resource="http://viaf.org/viaf/151962300"/>
    <dc:contributor xml:lang="en">Metadata Management Associates</dc:contributor>
    <dct:issued>2023</dct:issued>
    <dc:language>en</dc:language>
    <dct:license rdf:resource="http://creativecommons.org/publicdomain/zero/1.0"/>
    <schema:version>1-1-0</schema:version>
    <dct:hasFormat rdf:resource="https://uwlib-cams.github.io/uwlswd_vocabs_marc_006_008/008/visual_type_of_visual_material/visual_type_of_visual_material.ttl"/>
    <dct:hasFormat rdf:resource="https://uwlib-cams.github.io/uwlswd_vocabs_marc_006_008/008/visual_type_of_visual_material/visual_type_of_visual_material.nt"/>
    <dct:hasFormat rdf:resource="https://uwlib-cams.github.io/uwlswd_vocabs_marc_006_008/008/visual_type_of_visual_material/visual_type_of_visual_material.jsonld"/>
    <dct:hasFormat rdf:resource="https://uwlib-cams.github.io/uwlswd_vocabs_marc_006_008/008/visual_type_of_visual_material/visual_type_of_visual_material.html"/>
    <dct:format rdf:resource="http://www.w3.org/ns/formats/RDF_XML"/>
  </rdf:Description>
  <rdf:Description rdf:about="https://doi.org/10.6069/uwlswd.qgc0-9r48#s">
    <rdf:type rdf:resource="http://www.w3.org/2004/02/skos/core#Concept"/>
    <skos:inScheme rdf:resource="https://doi.org/10.6069/uwlswd.qgc0-9r48"/>
    <skos:prefLabel xml:lang="en">slide</skos:prefLabel>
    <skos:definition xml:lang="en">Transparent material on which there is a two-dimensional image, usually held in a mount, and designed for use in a projector or viewer.</skos:definition>
    <skos:notation>s</skos:notation>
    <skos:scopeNote xml:lang="en">Modern stereographs, for example, Viewmaster reels, are included here.</skos:scopeNote>
  </rdf:Description>
  <rdf:Description rdf:about="https://doi.org/10.6069/uwlswd.qgc0-9r48#c">
    <rdf:type rdf:resource="http://www.w3.org/2004/02/skos/core#Concept"/>
    <skos:inScheme rdf:resource="https://doi.org/10.6069/uwlswd.qgc0-9r48"/>
    <skos:prefLabel xml:lang="en">art reproduction</skos:prefLabel>
    <skos:definition xml:lang="en">Two or three-dimensional mechanically reproduced copy of a work of art, generally as one of a commercial edition.</skos:definition>
    <skos:notation>c</skos:notation>
  </rdf:Description>
  <rdf:Description rdf:about="https://doi.org/10.6069/uwlswd.qgc0-9r48#r">
    <rdf:type rdf:resource="http://www.w3.org/2004/02/skos/core#Concept"/>
    <skos:inScheme rdf:resource="https://doi.org/10.6069/uwlswd.qgc0-9r48"/>
    <skos:prefLabel xml:lang="en">realia</skos:prefLabel>
    <skos:definition xml:lang="en">Realia.</skos:definition>
    <skos:notation>r</skos:notation>
    <skos:scopeNote xml:lang="en">Includes 1) all three-dimensional items such as clothing, stitchery, fabrics, tools, and utensils; and 2) naturally occurring objects.</skos:scopeNote>
  </rdf:Description>
  <rdf:Description rdf:about="https://doi.org/10.6069/uwlswd.qgc0-9r48#t">
    <rdf:type rdf:resource="http://www.w3.org/2004/02/skos/core#Concept"/>
    <skos:inScheme rdf:resource="https://doi.org/10.6069/uwlswd.qgc0-9r48"/>
    <skos:prefLabel xml:lang="en">transparency</skos:prefLabel>
    <skos:definition xml:lang="en">Transparent material on which a basically still image is recorded. Transparencies are designed for use with an overhead projector or a light box.</skos:definition>
    <skos:notation>t</skos:notation>
    <skos:scopeNote xml:lang="en">X-rays are coded as transparencies.</skos:scopeNote>
  </rdf:Description>
  <rdf:Description rdf:about="https://doi.org/10.6069/uwlswd.qgc0-9r48#k">
    <rdf:type rdf:resource="http://www.w3.org/2004/02/skos/core#Concept"/>
    <skos:inScheme rdf:resource="https://doi.org/10.6069/uwlswd.qgc0-9r48"/>
    <skos:prefLabel xml:lang="en">graphic</skos:prefLabel>
    <skos:definition xml:lang="en">Graphic.</skos:definition>
    <skos:scopeNote xml:lang="en">Used for original or historical graphic material.</skos:scopeNote>
    <skos:notation>k</skos:notation>
  </rdf:Description>
  <rdf:Description rdf:about="https://doi.org/10.6069/uwlswd.qgc0-9r48#o">
    <rdf:type rdf:resource="http://www.w3.org/2004/02/skos/core#Concept"/>
    <skos:inScheme rdf:resource="https://doi.org/10.6069/uwlswd.qgc0-9r48"/>
    <skos:prefLabel xml:lang="en">flash card</skos:prefLabel>
    <skos:definition xml:lang="en">Card or other opaque material printed with words, numerals, or pictures and designed for rapid display.</skos:definition>
    <skos:notation>o</skos:notation>
    <skos:scopeNote xml:lang="en">Activity cards are included in this category.</skos:scopeNote>
  </rdf:Description>
  <rdf:Description rdf:about="https://doi.org/10.6069/uwlswd.qgc0-9r48#q">
    <rdf:type rdf:resource="http://www.w3.org/2004/02/skos/core#Concept"/>
    <skos:inScheme rdf:resource="https://doi.org/10.6069/uwlswd.qgc0-9r48"/>
    <skos:prefLabel xml:lang="en">model</skos:prefLabel>
    <skos:definition xml:lang="en">Three-dimensional representation of a real thing, either of the exact size of the original or to scale.</skos:definition>
    <skos:notation>q</skos:notation>
  </rdf:Description>
  <rdf:Description rdf:about="https://doi.org/10.6069/uwlswd.qgc0-9r48#a">
    <rdf:type rdf:resource="http://www.w3.org/2004/02/skos/core#Concept"/>
    <skos:inScheme rdf:resource="https://doi.org/10.6069/uwlswd.qgc0-9r48"/>
    <skos:prefLabel xml:lang="en">art original</skos:prefLabel>
    <skos:definition xml:lang="en">Two or three-dimensional work of art created by an artist, for example, a sculpture, as contrasted with a reproduction of it.</skos:definition>
    <skos:notation>a</skos:notation>
  </rdf:Description>
  <rdf:Description rdf:about="https://doi.org/10.6069/uwlswd.qgc0-9r48#p">
    <rdf:type rdf:resource="http://www.w3.org/2004/02/skos/core#Concept"/>
    <skos:inScheme rdf:resource="https://doi.org/10.6069/uwlswd.qgc0-9r48"/>
    <skos:prefLabel xml:lang="en">microscope slide</skos:prefLabel>
    <skos:definition xml:lang="en">Transparent mount, usually glass, containing a minute object to be viewed through a microscope or microprojector.</skos:definition>
    <skos:notation>p</skos:notation>
  </rdf:Description>
  <rdf:Description rdf:about="https://doi.org/10.6069/uwlswd.qgc0-9r48#i">
    <rdf:type rdf:resource="http://www.w3.org/2004/02/skos/core#Concept"/>
    <skos:inScheme rdf:resource="https://doi.org/10.6069/uwlswd.qgc0-9r48"/>
    <skos:prefLabel xml:lang="en">picture</skos:prefLabel>
    <skos:definition xml:lang="en">Two-dimensional visual representation accessible to the naked eye and generally on an opaque backing.</skos:definition>
    <skos:notation>i</skos:notation>
  </rdf:Description>
  <rdf:Description rdf:about="https://doi.org/10.6069/uwlswd.qgc0-9r48#l">
    <rdf:type rdf:resource="http://www.w3.org/2004/02/skos/core#Concept"/>
    <skos:inScheme rdf:resource="https://doi.org/10.6069/uwlswd.qgc0-9r48"/>
    <skos:prefLabel xml:lang="en">technical drawing</skos:prefLabel>
    <skos:definition xml:lang="en">Cross section, detail, diagram, elevation, perspective, plan, working plan, etc., made for use in an architectural engineering or other technical context.</skos:definition>
    <skos:notation>l</skos:notation>
  </rdf:Description>
  <rdf:Description rdf:about="https://doi.org/10.6069/uwlswd.qgc0-9r48#b">
    <rdf:type rdf:resource="http://www.w3.org/2004/02/skos/core#Concept"/>
    <skos:inScheme rdf:resource="https://doi.org/10.6069/uwlswd.qgc0-9r48"/>
    <skos:prefLabel xml:lang="en">kit</skos:prefLabel>
    <skos:definition xml:lang="en">Mixture of components from two or more categories, that is, sound recording, maps, filmstrips, etc., no one of which is the predominant constituent of the item.</skos:definition>
    <skos:notation>b</skos:notation>
    <skos:scopeNote xml:lang="en">Also includes the packages of material called laboratory kits, and packages of assorted materials, such as a set of K-12 social studies curriculum material (all books, workbooks, guides, activities, etc.) or packages of educational test materials (tests, answer sheets, scoring guides, score charts, interpretative manuals, etc.).</skos:scopeNote>
  </rdf:Description>
  <rdf:Description rdf:about="https://doi.org/10.6069/uwlswd.qgc0-9r48#z">
    <rdf:type rdf:resource="http://www.w3.org/2004/02/skos/core#Concept"/>
    <skos:inScheme rdf:resource="https://doi.org/10.6069/uwlswd.qgc0-9r48"/>
    <skos:prefLabel xml:lang="en">other</skos:prefLabel>
    <skos:definition xml:lang="en">Type of visual material other than art original, kit, art reproduction, diorama, filmstrip, game, picture, graphic, technical drawing, motion picture, chart, flash card, microscope slide, model, realia, slide, transparency, videorecording, or toy.</skos:definition>
    <skos:notation>z</skos:notation>
  </rdf:Description>
  <rdf:Description rdf:about="https://doi.org/10.6069/uwlswd.qgc0-9r48#v">
    <rdf:type rdf:resource="http://www.w3.org/2004/02/skos/core#Concept"/>
    <skos:inScheme rdf:resource="https://doi.org/10.6069/uwlswd.qgc0-9r48"/>
    <skos:prefLabel xml:lang="en">videorecording</skos:prefLabel>
    <skos:definition xml:lang="en">Recording on which visual images, usually in motion and accompanied by sound, have been registered. Videorecordings are designed for playback by means of a television receiver or monitor.</skos:definition>
    <skos:notation>v</skos:notation>
  </rdf:Description>
  <rdf:Description rdf:about="https://doi.org/10.6069/uwlswd.qgc0-9r48#n">
    <rdf:type rdf:resource="http://www.w3.org/2004/02/skos/core#Concept"/>
    <skos:inScheme rdf:resource="https://doi.org/10.6069/uwlswd.qgc0-9r48"/>
    <skos:prefLabel xml:lang="en">chart</skos:prefLabel>
    <skos:definition xml:lang="en">Opaque sheet that exhibits data in graphic or tabular form (e.g., a calendar).</skos:definition>
    <skos:notation>n</skos:notation>
  </rdf:Description>
  <rdf:Description rdf:about="https://doi.org/10.6069/uwlswd.qgc0-9r48#w">
    <rdf:type rdf:resource="http://www.w3.org/2004/02/skos/core#Concept"/>
    <skos:inScheme rdf:resource="https://doi.org/10.6069/uwlswd.qgc0-9r48"/>
    <skos:prefLabel xml:lang="en">toy</skos:prefLabel>
    <skos:definition xml:lang="en">Material object for children or others to play with (often an imitation of some familiar object); a plaything; also, something contrived for amusement rather than for practical use.</skos:definition>
    <skos:notation>w</skos:notation>
  </rdf:Description>
  <rdf:Description rdf:about="https://doi.org/10.6069/uwlswd.qgc0-9r48#f">
    <rdf:type rdf:resource="http://www.w3.org/2004/02/skos/core#Concept"/>
    <skos:inScheme rdf:resource="https://doi.org/10.6069/uwlswd.qgc0-9r48"/>
    <skos:prefLabel xml:lang="en">filmstrip</skos:prefLabel>
    <skos:definition xml:lang="en">Length of film containing a succession of images intended for projection one frame at a time with or without recorded sound.</skos:definition>
    <skos:notation>f</skos:notation>
  </rdf:Description>
  <rdf:Description rdf:about="https://doi.org/10.6069/uwlswd.qgc0-9r48#m">
    <rdf:type rdf:resource="http://www.w3.org/2004/02/skos/core#Concept"/>
    <skos:inScheme rdf:resource="https://doi.org/10.6069/uwlswd.qgc0-9r48"/>
    <skos:prefLabel xml:lang="en">motion picture</skos:prefLabel>
    <skos:definition xml:lang="en">Series of still pictures on film with or without sound, designed to be projected in rapid succession to produce the optical effect of motion.</skos:definition>
    <skos:notation>m</skos:notation>
  </rdf:Description>
  <rdf:Description rdf:about="https://doi.org/10.6069/uwlswd.qgc0-9r48#ex">
    <rdf:type rdf:resource="http://www.w3.org/2004/02/skos/core#Concept"/>
    <skos:inScheme rdf:resource="https://doi.org/10.6069/uwlswd.qgc0-9r48"/>
    <skos:prefLabel xml:lang="en">electronic videorecording [obsolete]</skos:prefLabel>
    <skos:notation>e</skos:notation>
  </rdf:Description>
  <rdf:Description rdf:about="https://doi.org/10.6069/uwlswd.qgc0-9r48#g">
    <rdf:type rdf:resource="http://www.w3.org/2004/02/skos/core#Concept"/>
    <skos:inScheme rdf:resource="https://doi.org/10.6069/uwlswd.qgc0-9r48"/>
    <skos:prefLabel xml:lang="en">game</skos:prefLabel>
    <skos:definition xml:lang="en">Item or set of items designed for play according to prescribed rules and intended for recreation or instruction.</skos:definition>
    <skos:notation>g</skos:notation>
    <skos:scopeNote xml:lang="en">includes puzzles and simulations.</skos:scopeNote>
  </rdf:Description>
  <rdf:Description rdf:about="https://doi.org/10.6069/uwlswd.qgc0-9r48#d">
    <rdf:type rdf:resource="http://www.w3.org/2004/02/skos/core#Concept"/>
    <skos:inScheme rdf:resource="https://doi.org/10.6069/uwlswd.qgc0-9r48"/>
    <skos:prefLabel xml:lang="en">diorama</skos:prefLabel>
    <skos:definition xml:lang="en">Three-dimensional representation of a scene created by placing objects, figures, etc. in front of a two-dimensional background.</skos:definition>
    <skos:notation>d</skos:notation>
  </rdf:Description>
</rdf:RDF>
