@prefix dc: <http://purl.org/dc/elements/1.1/> .
@prefix dct: <http://purl.org/dc/terms/> .
@prefix schema: <https://schema.org/> .
@prefix skos: <http://www.w3.org/2004/02/skos/core#> .

<https://doi.org/10.6069/uwlswd.fr5p-1828#a> a skos:Concept ;
    skos:definition "Microfilm."@en ;
    skos:inScheme <https://doi.org/10.6069/uwlswd.fr5p-1828> ;
    skos:notation "a" ;
    skos:prefLabel "microfilm"@en .

<https://doi.org/10.6069/uwlswd.fr5p-1828#b> a skos:Concept ;
    skos:definition "Microfiche."@en ;
    skos:inScheme <https://doi.org/10.6069/uwlswd.fr5p-1828> ;
    skos:notation "b" ;
    skos:prefLabel "microfiche"@en .

<https://doi.org/10.6069/uwlswd.fr5p-1828#c> a skos:Concept ;
    skos:definition "Microopaque."@en ;
    skos:inScheme <https://doi.org/10.6069/uwlswd.fr5p-1828> ;
    skos:notation "c" ;
    skos:prefLabel "microopaque"@en .

<https://doi.org/10.6069/uwlswd.fr5p-1828#d> a skos:Concept ;
    skos:definition "Large print."@en ;
    skos:inScheme <https://doi.org/10.6069/uwlswd.fr5p-1828> ;
    skos:notation "d" ;
    skos:prefLabel "large print"@en .

<https://doi.org/10.6069/uwlswd.fr5p-1828#f> a skos:Concept ;
    skos:definition "Braille."@en ;
    skos:inScheme <https://doi.org/10.6069/uwlswd.fr5p-1828> ;
    skos:notation "f" ;
    skos:prefLabel "braille"@en .

<https://doi.org/10.6069/uwlswd.fr5p-1828#o> a skos:Concept ;
    skos:definition "Accessed by means of hardware and software connections to a communications network."@en ;
    skos:inScheme <https://doi.org/10.6069/uwlswd.fr5p-1828> ;
    skos:notation "o" ;
    skos:prefLabel "online"@en .

<https://doi.org/10.6069/uwlswd.fr5p-1828#pound> a skos:Concept ;
    skos:definition "Form of item other than microfilm, microfiche, microopaque, large print, braille, online, direct electronic, regular print reproduction, or electronic."@en ;
    skos:inScheme <https://doi.org/10.6069/uwlswd.fr5p-1828> ;
    skos:notation "#" ;
    skos:prefLabel "none of the following"@en ;
    skos:scopeNote "Not specified by one of the other codes."@en .

<https://doi.org/10.6069/uwlswd.fr5p-1828#q> a skos:Concept ;
    skos:definition "Storage on a directly accessible tangible recording medium, e.g. disc, tape, playaway device, flashdrive, portable hard drive, etc."@en ;
    skos:inScheme <https://doi.org/10.6069/uwlswd.fr5p-1828> ;
    skos:notation "q" ;
    skos:prefLabel "direct electronic"@en .

<https://doi.org/10.6069/uwlswd.fr5p-1828#r> a skos:Concept ;
    skos:definition "Eye-readable print, such as a photocopy." ;
    skos:inScheme <https://doi.org/10.6069/uwlswd.fr5p-1828> ;
    skos:notation "r" ;
    skos:prefLabel "regular print reproduction"@en .

<https://doi.org/10.6069/uwlswd.fr5p-1828#s> a skos:Concept ;
    skos:definition "Intended for manipulation by a computer. May reside in a carrier accessed either directly or remotely, in some cases requiring the use of peripheral devices attached to the computer (e.g., a CD-ROM player)."@en ;
    skos:inScheme <https://doi.org/10.6069/uwlswd.fr5p-1828> ;
    skos:notation "s" ;
    skos:prefLabel "electronic"@en ;
    skos:scopeNote "Not used for items that do not require the use of a computer (e.g., music compact discs, videodiscs)."@en .

<https://doi.org/10.6069/uwlswd.fr5p-1828> a skos:ConceptScheme ;
    dc:contributor "Metadata Management Associates"@en ;
    dc:language "en" ;
    dct:alternative "MARC21 008/29 values for visual materials expressed using RDF"@en ;
    dct:contributor <http://viaf.org/viaf/151962300> ;
    dct:creator <http://viaf.org/viaf/139541794> ;
    dct:description "Specifies the form of material."@en ;
    dct:format <http://www.w3.org/ns/formats/Turtle> ;
    dct:hasFormat <https://uwlib-cams.github.io/uwlswd_vocabs_marc_006_008/008/visual_form_of_item/visual_form_of_item.html>,
        <https://uwlib-cams.github.io/uwlswd_vocabs_marc_006_008/008/visual_form_of_item/visual_form_of_item.jsonld>,
        <https://uwlib-cams.github.io/uwlswd_vocabs_marc_006_008/008/visual_form_of_item/visual_form_of_item.nt>,
        <https://uwlib-cams.github.io/uwlswd_vocabs_marc_006_008/008/visual_form_of_item/visual_form_of_item.rdf> ;
    dct:issued "2024" ;
    dct:license <http://creativecommons.org/publicdomain/zero/1.0> ;
    dct:provenance <https://doi.org/10.6069/uwlswd.2e2b-y833> ;
    dct:publisher <http://viaf.org/viaf/139541794> ;
    dct:source <http://marc21rdf.info>,
        <https://www.loc.gov/marc/bibliographic/bd008.html> ;
    dct:title "Visual: form of item"@en ;
    dct:type <http://purl.org/dc/dcmitype/Dataset> ;
    schema:disambiguatingDescription "SKOS Concept Scheme for MARC 00X Values"@en ;
    schema:version "1-0-0" .

