<?xml version="1.0" encoding="utf-8"?>
<rdf:RDF
   xmlns:dc="http://purl.org/dc/elements/1.1/"
   xmlns:dct="http://purl.org/dc/terms/"
   xmlns:rdf="http://www.w3.org/1999/02/22-rdf-syntax-ns#"
   xmlns:schema="https://schema.org/"
   xmlns:skos="http://www.w3.org/2004/02/skos/core#"
>
  <rdf:Description rdf:about="https://doi.org/10.6069/uwlswd.fr5p-1828#pound">
    <rdf:type rdf:resource="http://www.w3.org/2004/02/skos/core#Concept"/>
    <skos:inScheme rdf:resource="https://doi.org/10.6069/uwlswd.fr5p-1828"/>
    <skos:prefLabel xml:lang="en">none of the following</skos:prefLabel>
    <skos:definition xml:lang="en">Form of item other than microfilm, microfiche, microopaque, large print, braille, online, direct electronic, regular print reproduction, or electronic.</skos:definition>
    <skos:notation>#</skos:notation>
    <skos:scopeNote xml:lang="en">Not specified by one of the other codes.</skos:scopeNote>
  </rdf:Description>
  <rdf:Description rdf:about="https://doi.org/10.6069/uwlswd.fr5p-1828#q">
    <rdf:type rdf:resource="http://www.w3.org/2004/02/skos/core#Concept"/>
    <skos:inScheme rdf:resource="https://doi.org/10.6069/uwlswd.fr5p-1828"/>
    <skos:prefLabel xml:lang="en">direct electronic</skos:prefLabel>
    <skos:definition xml:lang="en">Storage on a directly accessible tangible recording medium, e.g. disc, tape, playaway device, flashdrive, portable hard drive, etc.</skos:definition>
    <skos:notation>q</skos:notation>
  </rdf:Description>
  <rdf:Description rdf:about="https://doi.org/10.6069/uwlswd.fr5p-1828#f">
    <rdf:type rdf:resource="http://www.w3.org/2004/02/skos/core#Concept"/>
    <skos:inScheme rdf:resource="https://doi.org/10.6069/uwlswd.fr5p-1828"/>
    <skos:prefLabel xml:lang="en">braille</skos:prefLabel>
    <skos:definition xml:lang="en">Braille.</skos:definition>
    <skos:notation>f</skos:notation>
  </rdf:Description>
  <rdf:Description rdf:about="https://doi.org/10.6069/uwlswd.fr5p-1828#s">
    <rdf:type rdf:resource="http://www.w3.org/2004/02/skos/core#Concept"/>
    <skos:inScheme rdf:resource="https://doi.org/10.6069/uwlswd.fr5p-1828"/>
    <skos:prefLabel xml:lang="en">electronic</skos:prefLabel>
    <skos:definition xml:lang="en">Intended for manipulation by a computer. May reside in a carrier accessed either directly or remotely, in some cases requiring the use of peripheral devices attached to the computer (e.g., a CD-ROM player).</skos:definition>
    <skos:notation>s</skos:notation>
    <skos:scopeNote xml:lang="en">Not used for items that do not require the use of a computer (e.g., music compact discs, videodiscs).</skos:scopeNote>
  </rdf:Description>
  <rdf:Description rdf:about="https://doi.org/10.6069/uwlswd.fr5p-1828#a">
    <rdf:type rdf:resource="http://www.w3.org/2004/02/skos/core#Concept"/>
    <skos:inScheme rdf:resource="https://doi.org/10.6069/uwlswd.fr5p-1828"/>
    <skos:prefLabel xml:lang="en">microfilm</skos:prefLabel>
    <skos:definition xml:lang="en">Microfilm.</skos:definition>
    <skos:notation>a</skos:notation>
  </rdf:Description>
  <rdf:Description rdf:about="https://doi.org/10.6069/uwlswd.fr5p-1828">
    <rdf:type rdf:resource="http://www.w3.org/2004/02/skos/core#ConceptScheme"/>
    <dct:type rdf:resource="http://purl.org/dc/dcmitype/Dataset"/>
    <dct:title xml:lang="en">Visual: form of item</dct:title>
    <dct:alternative xml:lang="en">MARC21 008/29 values for visual materials expressed using RDF</dct:alternative>
    <dct:description xml:lang="en">Specifies the form of material.</dct:description>
    <schema:disambiguatingDescription xml:lang="en">SKOS Concept Scheme for MARC 00X Values</schema:disambiguatingDescription>
    <dct:publisher rdf:resource="http://viaf.org/viaf/139541794"/>
    <dct:source rdf:resource="https://www.loc.gov/marc/bibliographic/bd008.html"/>
    <dct:source rdf:resource="http://marc21rdf.info"/>
    <dct:provenance rdf:resource="https://doi.org/10.6069/uwlswd.2e2b-y833#marc00Xvalues"/>
    <dct:creator rdf:resource="http://viaf.org/viaf/139541794"/>
    <dct:contributor rdf:resource="http://viaf.org/viaf/151962300"/>
    <dc:contributor xml:lang="en">Metadata Management Associates</dc:contributor>
    <dct:issued>2024</dct:issued>
    <dc:language>en</dc:language>
    <dct:license rdf:resource="http://creativecommons.org/publicdomain/zero/1.0"/>
    <schema:version>1-1-0</schema:version>
    <dct:format rdf:resource="http://www.w3.org/ns/formats/RDF_XML"/>
    <dct:hasFormat rdf:resource="https://uwlib-cams.github.io/uwlswd_vocabs_marc_006_008/008/visual_form_of_item/visual_form_of_item.ttl"/>
    <dct:hasFormat rdf:resource="https://uwlib-cams.github.io/uwlswd_vocabs_marc_006_008/008/visual_form_of_item/visual_form_of_item.nt"/>
    <dct:hasFormat rdf:resource="https://uwlib-cams.github.io/uwlswd_vocabs_marc_006_008/008/visual_form_of_item/visual_form_of_item.jsonld"/>
    <dct:hasFormat rdf:resource="https://uwlib-cams.github.io/uwlswd_vocabs_marc_006_008/008/visual_form_of_item/visual_form_of_item.html"/>
  </rdf:Description>
  <rdf:Description rdf:about="https://doi.org/10.6069/uwlswd.fr5p-1828#r">
    <rdf:type rdf:resource="http://www.w3.org/2004/02/skos/core#Concept"/>
    <skos:inScheme rdf:resource="https://doi.org/10.6069/uwlswd.fr5p-1828"/>
    <skos:prefLabel xml:lang="en">regular print reproduction</skos:prefLabel>
    <skos:definition>Eye-readable print, such as a photocopy.</skos:definition>
    <skos:notation>r</skos:notation>
  </rdf:Description>
  <rdf:Description rdf:about="https://doi.org/10.6069/uwlswd.fr5p-1828#o">
    <rdf:type rdf:resource="http://www.w3.org/2004/02/skos/core#Concept"/>
    <skos:inScheme rdf:resource="https://doi.org/10.6069/uwlswd.fr5p-1828"/>
    <skos:prefLabel xml:lang="en">online</skos:prefLabel>
    <skos:definition xml:lang="en">Accessed by means of hardware and software connections to a communications network.</skos:definition>
    <skos:notation>o</skos:notation>
  </rdf:Description>
  <rdf:Description rdf:about="https://doi.org/10.6069/uwlswd.fr5p-1828#b">
    <rdf:type rdf:resource="http://www.w3.org/2004/02/skos/core#Concept"/>
    <skos:inScheme rdf:resource="https://doi.org/10.6069/uwlswd.fr5p-1828"/>
    <skos:prefLabel xml:lang="en">microfiche</skos:prefLabel>
    <skos:definition xml:lang="en">Microfiche.</skos:definition>
    <skos:notation>b</skos:notation>
  </rdf:Description>
  <rdf:Description rdf:about="https://doi.org/10.6069/uwlswd.fr5p-1828#c">
    <rdf:type rdf:resource="http://www.w3.org/2004/02/skos/core#Concept"/>
    <skos:inScheme rdf:resource="https://doi.org/10.6069/uwlswd.fr5p-1828"/>
    <skos:prefLabel xml:lang="en">microopaque</skos:prefLabel>
    <skos:definition xml:lang="en">Microopaque.</skos:definition>
    <skos:notation>c</skos:notation>
  </rdf:Description>
  <rdf:Description rdf:about="https://doi.org/10.6069/uwlswd.fr5p-1828#d">
    <rdf:type rdf:resource="http://www.w3.org/2004/02/skos/core#Concept"/>
    <skos:inScheme rdf:resource="https://doi.org/10.6069/uwlswd.fr5p-1828"/>
    <skos:prefLabel xml:lang="en">large print</skos:prefLabel>
    <skos:definition xml:lang="en">Large print.</skos:definition>
    <skos:notation>d</skos:notation>
  </rdf:Description>
</rdf:RDF>
