<?xml version='1.0' encoding='UTF-8'?>
<rdf:RDF xmlns:dc="http://purl.org/dc/elements/1.1/" xmlns:dct="http://purl.org/dc/terms/" xmlns:rdf="http://www.w3.org/1999/02/22-rdf-syntax-ns#" xmlns:schema="https://schema.org/" xmlns:skos="http://www.w3.org/2004/02/skos/core#">
  <rdf:Description rdf:about="https://doi.org/10.6069/uwlswd.vw5v-gh79">
    <rdf:type rdf:resource="http://www.w3.org/2004/02/skos/core#ConceptScheme"/>
    <dct:type rdf:resource="http://purl.org/dc/dcmitype/Dataset"/>
    <dct:title xml:lang="en">Maps: type of cartographic material</dct:title>
    <dct:alternative xml:lang="en">MARC21 008/25 values for maps expressed using RDF</dct:alternative>
    <dct:description xml:lang="en">Indicates the type of cartographic item described.</dct:description>
    <schema:disambiguatingDescription xml:lang="en">SKOS Concept Scheme for MARC 00X Values</schema:disambiguatingDescription>
    <dct:publisher rdf:resource="http://viaf.org/viaf/139541794"/>
    <dct:source rdf:resource="https://www.loc.gov/marc/bibliographic/bd008.html"/>
    <dct:source rdf:resource="http://marc21rdf.info"/>
    <dct:provenance rdf:resource="https://doi.org/10.6069/uwlswd.2e2b-y833"/>
    <dct:creator rdf:resource="http://viaf.org/viaf/139541794"/>
    <dct:contributor rdf:resource="http://viaf.org/viaf/151962300"/>
    <dc:contributor xml:lang="en">Metadata Management Associates</dc:contributor>
    <dct:issued>2023</dct:issued>
    <dc:language>en</dc:language>
    <dct:license rdf:resource="http://creativecommons.org/publicdomain/zero/1.0"/>
    <schema:version>1-0-1</schema:version>
    <dct:hasFormat rdf:resource="https://uwlib-cams.github.io/uwlswd_vocabs_marc_006_008/008/maps_type_of_cartographic_material/maps_type_of_cartographic_material.ttl"/>
    <dct:hasFormat rdf:resource="https://uwlib-cams.github.io/uwlswd_vocabs_marc_006_008/008/maps_type_of_cartographic_material/maps_type_of_cartographic_material.nt"/>
    <dct:hasFormat rdf:resource="https://uwlib-cams.github.io/uwlswd_vocabs_marc_006_008/008/maps_type_of_cartographic_material/maps_type_of_cartographic_material.jsonld"/>
    <dct:hasFormat rdf:resource="https://uwlib-cams.github.io/uwlswd_vocabs_marc_006_008/008/maps_type_of_cartographic_material/maps_type_of_cartographic_material.html"/>
    <dct:format rdf:resource="http://www.w3.org/ns/formats/RDF_XML"/>
  </rdf:Description>
  <rdf:Description rdf:about="https://doi.org/10.6069/uwlswd.vw5v-gh79#f">
    <rdf:type rdf:resource="http://www.w3.org/2004/02/skos/core#Concept"/>
    <skos:inScheme rdf:resource="https://doi.org/10.6069/uwlswd.vw5v-gh79"/>
    <skos:prefLabel xml:lang="en">separate supplement to another work</skos:prefLabel>
    <skos:definition xml:lang="en">Separate supplement to another work</skos:definition>
    <skos:notation>f</skos:notation>
    <skos:scopeNote xml:lang="en">Other work being supplemented does not have to be cartographic material.</skos:scopeNote>
  </rdf:Description>
  <rdf:Description rdf:about="https://doi.org/10.6069/uwlswd.vw5v-gh79#g">
    <rdf:type rdf:resource="http://www.w3.org/2004/02/skos/core#Concept"/>
    <skos:inScheme rdf:resource="https://doi.org/10.6069/uwlswd.vw5v-gh79"/>
    <skos:prefLabel xml:lang="en">bound as part of another work</skos:prefLabel>
    <skos:definition xml:lang="en">Bound as part of another work</skos:definition>
    <skos:notation>g</skos:notation>
    <skos:scopeNote xml:lang="en">Other work included does not have to be cartographic material.</skos:scopeNote>
  </rdf:Description>
  <rdf:Description rdf:about="https://doi.org/10.6069/uwlswd.vw5v-gh79#c">
    <rdf:type rdf:resource="http://www.w3.org/2004/02/skos/core#Concept"/>
    <skos:inScheme rdf:resource="https://doi.org/10.6069/uwlswd.vw5v-gh79"/>
    <skos:prefLabel xml:lang="en">map serial</skos:prefLabel>
    <skos:definition xml:lang="en">Issued in successive parts bearing numerical or chronological designations and intended to be continued indefinitely.</skos:definition>
    <skos:notation>c</skos:notation>
    <skos:scopeNote xml:lang="en">Not used for serially issued atlases.</skos:scopeNote>
  </rdf:Description>
  <rdf:Description rdf:about="https://doi.org/10.6069/uwlswd.vw5v-gh79#a">
    <rdf:type rdf:resource="http://www.w3.org/2004/02/skos/core#Concept"/>
    <skos:inScheme rdf:resource="https://doi.org/10.6069/uwlswd.vw5v-gh79"/>
    <skos:prefLabel xml:lang="en">single map</skos:prefLabel>
    <skos:definition xml:lang="en">Single map.</skos:definition>
    <skos:notation>a</skos:notation>
  </rdf:Description>
  <rdf:Description rdf:about="https://doi.org/10.6069/uwlswd.vw5v-gh79#e">
    <rdf:type rdf:resource="http://www.w3.org/2004/02/skos/core#Concept"/>
    <skos:inScheme rdf:resource="https://doi.org/10.6069/uwlswd.vw5v-gh79"/>
    <skos:prefLabel xml:lang="en">atlas</skos:prefLabel>
    <skos:definition xml:lang="en">Atlas.</skos:definition>
    <skos:notation>e</skos:notation>
    <skos:scopeNote xml:lang="en">Includes atlas series, and serially issued atlases.</skos:scopeNote>
  </rdf:Description>
  <rdf:Description rdf:about="https://doi.org/10.6069/uwlswd.vw5v-gh79#b">
    <rdf:type rdf:resource="http://www.w3.org/2004/02/skos/core#Concept"/>
    <skos:inScheme rdf:resource="https://doi.org/10.6069/uwlswd.vw5v-gh79"/>
    <skos:prefLabel xml:lang="en">map series</skos:prefLabel>
    <skos:definition xml:lang="en">Number of related but physically separate and bibliographically distinct cartographic units intended by the producer(s) or issuing body(s) to form a single group.</skos:definition>
    <skos:notation>b</skos:notation>
    <skos:scopeNote xml:lang="en">Not used for atlas series.</skos:scopeNote>
  </rdf:Description>
  <rdf:Description rdf:about="https://doi.org/10.6069/uwlswd.vw5v-gh79#z">
    <rdf:type rdf:resource="http://www.w3.org/2004/02/skos/core#Concept"/>
    <skos:inScheme rdf:resource="https://doi.org/10.6069/uwlswd.vw5v-gh79"/>
    <skos:prefLabel xml:lang="en">other</skos:prefLabel>
    <skos:definition xml:lang="en">Type of cartographic material other than single map, map series, map serial, globe, atlas, separate map supplement to another work, or map bound as part of another work.</skos:definition>
    <skos:notation>z</skos:notation>
  </rdf:Description>
  <rdf:Description rdf:about="https://doi.org/10.6069/uwlswd.vw5v-gh79#d">
    <rdf:type rdf:resource="http://www.w3.org/2004/02/skos/core#Concept"/>
    <skos:inScheme rdf:resource="https://doi.org/10.6069/uwlswd.vw5v-gh79"/>
    <skos:prefLabel xml:lang="en">globe</skos:prefLabel>
    <skos:definition xml:lang="en">Globe.</skos:definition>
    <skos:notation>d</skos:notation>
  </rdf:Description>
  <rdf:Description rdf:about="https://doi.org/10.6069/uwlswd.vw5v-gh79#u">
    <rdf:type rdf:resource="http://www.w3.org/2004/02/skos/core#Concept"/>
    <skos:inScheme rdf:resource="https://doi.org/10.6069/uwlswd.vw5v-gh79"/>
    <skos:prefLabel xml:lang="en">unknown</skos:prefLabel>
    <skos:definition xml:lang="en">Unknown.</skos:definition>
    <skos:notation>u</skos:notation>
  </rdf:Description>
</rdf:RDF>