<?xml version='1.0' encoding='UTF-8'?>
<rdf:RDF xmlns:dc="http://purl.org/dc/elements/1.1/" xmlns:dct="http://purl.org/dc/terms/" xmlns:rdf="http://www.w3.org/1999/02/22-rdf-syntax-ns#" xmlns:schema="https://schema.org/" xmlns:skos="http://www.w3.org/2004/02/skos/core#" xmlns:uwp="https://doi.org/10.6069/uwlib.55.d.3#">
  <rdf:Description rdf:about="https://doi.org/10.6069/uwlswd.2eg3-1x53#pound">
    <rdf:type rdf:resource="http://www.w3.org/2004/02/skos/core#Concept"/>
    <skos:inScheme rdf:resource="https://doi.org/10.6069/uwlswd.2eg3-1x53"/>
    <skos:prefLabel xml:lang="en">not a government publication</skos:prefLabel>
    <skos:definition xml:lang="en">Not published by or for a government body.</skos:definition>
    <skos:notation>#</skos:notation>
  </rdf:Description>
  <rdf:Description rdf:about="https://doi.org/10.6069/uwlswd.2eg3-1x53">
    <rdf:type rdf:resource="http://www.w3.org/2004/02/skos/core#ConceptScheme"/>
    <dct:type rdf:resource="http://purl.org/dc/dcmitype/Dataset"/>
    <dct:title xml:lang="en">Some: government publication</dct:title>
    <dct:alternative xml:lang="en">MARC21 008/28 values for some materials expressed using RDF</dct:alternative>
    <dct:description xml:lang="en">Indicates whether the item is published or produced by or for an international, provincial, national, state, or local government agency, or by any subdivision of such a body, and, if so, the jurisdictional level of the agency.</dct:description>
    <schema:disambiguatingDescription xml:lang="en">SKOS Concept Scheme for MARC 00X Values</schema:disambiguatingDescription>
    <dct:publisher rdf:resource="http://viaf.org/viaf/139541794"/>
    <dct:source rdf:resource="https://www.loc.gov/marc/bibliographic/bd008.html"/>
    <dct:source rdf:resource="http://marc21rdf.info"/>
    <dct:provenance rdf:resource="https://doi.org/10.6069/uwlswd.2e2b-y833#marc00Xvalues"/>
    <dct:creator rdf:resource="http://viaf.org/viaf/139541794"/>
    <dct:contributor rdf:resource="http://viaf.org/viaf/151962300"/>
    <dc:contributor xml:lang="en">Metadata Management Associates</dc:contributor>
    <dct:issued>2023</dct:issued>
    <dc:language>en</dc:language>
    <dct:license rdf:resource="http://creativecommons.org/publicdomain/zero/1.0"/>
    <schema:version>1-0-2</schema:version>
    <dct:hasFormat rdf:resource="https://uwlib-cams.github.io/uwlswd_vocabs_marc_006_008/008/some_government_publication/some_government_publication.ttl"/>
    <dct:hasFormat rdf:resource="https://uwlib-cams.github.io/uwlswd_vocabs_marc_006_008/008/some_government_publication/some_government_publication.nt"/>
    <dct:hasFormat rdf:resource="https://uwlib-cams.github.io/uwlswd_vocabs_marc_006_008/008/some_government_publication/some_government_publication.jsonld"/>
    <dct:hasFormat rdf:resource="https://uwlib-cams.github.io/uwlswd_vocabs_marc_006_008/008/some_government_publication/some_government_publication.html"/>
    <dct:format rdf:resource="http://www.w3.org/ns/formats/RDF_XML"/>
    <uwp:appliesToMaterial>books</uwp:appliesToMaterial>
    <uwp:appliesToMaterial>computer files</uwp:appliesToMaterial>
    <uwp:appliesToMaterial>maps</uwp:appliesToMaterial>
    <uwp:appliesToMaterial>continuing resources</uwp:appliesToMaterial>
    <uwp:appliesToMaterial>visual materials</uwp:appliesToMaterial>
  </rdf:Description>
  <rdf:Description rdf:about="https://doi.org/10.6069/uwlswd.2eg3-1x53#f">
    <rdf:type rdf:resource="http://www.w3.org/2004/02/skos/core#Concept"/>
    <skos:inScheme rdf:resource="https://doi.org/10.6069/uwlswd.2eg3-1x53"/>
    <skos:prefLabel xml:lang="en">federal or national</skos:prefLabel>
    <skos:definition xml:lang="en">Published or produced by or for a federal or national government body (e.g., a sovereign nation, such as Canada). Used for the governments of England, Wales, Scotland, and Northern Ireland. Also used for American Indian tribes.</skos:definition>
    <skos:notation>f</skos:notation>
  </rdf:Description>
  <rdf:Description rdf:about="https://doi.org/10.6069/uwlswd.2eg3-1x53#m">
    <rdf:type rdf:resource="http://www.w3.org/2004/02/skos/core#Concept"/>
    <skos:inScheme rdf:resource="https://doi.org/10.6069/uwlswd.2eg3-1x53"/>
    <skos:prefLabel xml:lang="en">multistate</skos:prefLabel>
    <skos:definition xml:lang="en">Published or produced by or for a regional combination of jurisdictions at the state, provincial, territorial, etc. level.</skos:definition>
    <skos:notation>m</skos:notation>
  </rdf:Description>
  <rdf:Description rdf:about="https://doi.org/10.6069/uwlswd.2eg3-1x53#i">
    <rdf:type rdf:resource="http://www.w3.org/2004/02/skos/core#Concept"/>
    <skos:inScheme rdf:resource="https://doi.org/10.6069/uwlswd.2eg3-1x53"/>
    <skos:prefLabel xml:lang="en">international intergovernmental</skos:prefLabel>
    <skos:definition xml:lang="en">Published or produced by or for an international intergovernmental body.</skos:definition>
    <skos:notation>i</skos:notation>
  </rdf:Description>
  <rdf:Description rdf:about="https://doi.org/10.6069/uwlswd.2eg3-1x53#z">
    <rdf:type rdf:resource="http://www.w3.org/2004/02/skos/core#Concept"/>
    <skos:inScheme rdf:resource="https://doi.org/10.6069/uwlswd.2eg3-1x53"/>
    <skos:prefLabel xml:lang="en">other</skos:prefLabel>
    <skos:definition xml:lang="en">Government publication other than autonomous or semi-autonomous component, multilocal, federal or national, international intergovernmental, local, multistate, government publication - level undetermined, state, provincial, territorial, or dependent.</skos:definition>
    <skos:notation>z</skos:notation>
  </rdf:Description>
  <rdf:Description rdf:about="https://doi.org/10.6069/uwlswd.2eg3-1x53#nx">
    <rdf:type rdf:resource="http://www.w3.org/2004/02/skos/core#Concept"/>
    <skos:inScheme rdf:resource="https://doi.org/10.6069/uwlswd.2eg3-1x53"/>
    <skos:prefLabel xml:lang="en">government publication - level undetermined [obsolete]</skos:prefLabel>
    <skos:notation>n</skos:notation>
  </rdf:Description>
  <rdf:Description rdf:about="https://doi.org/10.6069/uwlswd.2eg3-1x53#s">
    <rdf:type rdf:resource="http://www.w3.org/2004/02/skos/core#Concept"/>
    <skos:inScheme rdf:resource="https://doi.org/10.6069/uwlswd.2eg3-1x53"/>
    <skos:prefLabel xml:lang="en">state, provincial, territorial, dependent, etc.</skos:prefLabel>
    <skos:definition xml:lang="en">Jurisdictional level of the government body is a state, province, territory, or other dependent jurisdiction.</skos:definition>
    <skos:notation>s</skos:notation>
  </rdf:Description>
  <rdf:Description rdf:about="https://doi.org/10.6069/uwlswd.2eg3-1x53#u">
    <rdf:type rdf:resource="http://www.w3.org/2004/02/skos/core#Concept"/>
    <skos:inScheme rdf:resource="https://doi.org/10.6069/uwlswd.2eg3-1x53"/>
    <skos:prefLabel xml:lang="en">unknown if item is government publication</skos:prefLabel>
    <skos:definition xml:lang="en">Whether or not the item is published or produced by or for a government agency is unknown.</skos:definition>
    <skos:notation>u</skos:notation>
  </rdf:Description>
  <rdf:Description rdf:about="https://doi.org/10.6069/uwlswd.2eg3-1x53#o">
    <rdf:type rdf:resource="http://www.w3.org/2004/02/skos/core#Concept"/>
    <skos:inScheme rdf:resource="https://doi.org/10.6069/uwlswd.2eg3-1x53"/>
    <skos:prefLabel xml:lang="en">government publication - level undetermined</skos:prefLabel>
    <skos:definition xml:lang="en">Published or produced by or for a government body but that the jurisdictional level cannot be determined.</skos:definition>
    <skos:notation>o</skos:notation>
  </rdf:Description>
  <rdf:Description rdf:about="https://doi.org/10.6069/uwlswd.2eg3-1x53#l">
    <rdf:type rdf:resource="http://www.w3.org/2004/02/skos/core#Concept"/>
    <skos:inScheme rdf:resource="https://doi.org/10.6069/uwlswd.2eg3-1x53"/>
    <skos:prefLabel xml:lang="en">local</skos:prefLabel>
    <skos:definition xml:lang="en">Published or produced by or for a local government jurisdiction such as a town, city, county, etc.</skos:definition>
    <skos:notation>l</skos:notation>
  </rdf:Description>
  <rdf:Description rdf:about="https://doi.org/10.6069/uwlswd.2eg3-1x53#a">
    <rdf:type rdf:resource="http://www.w3.org/2004/02/skos/core#Concept"/>
    <skos:inScheme rdf:resource="https://doi.org/10.6069/uwlswd.2eg3-1x53"/>
    <skos:prefLabel xml:lang="en">autonomous or semi-autonomous component</skos:prefLabel>
    <skos:definition xml:lang="en">Published or produced by or for a government body of an autonomous or semi-autonomous component of a country.</skos:definition>
    <skos:notation>a</skos:notation>
  </rdf:Description>
  <rdf:Description rdf:about="https://doi.org/10.6069/uwlswd.2eg3-1x53#c">
    <rdf:type rdf:resource="http://www.w3.org/2004/02/skos/core#Concept"/>
    <skos:inScheme rdf:resource="https://doi.org/10.6069/uwlswd.2eg3-1x53"/>
    <skos:prefLabel xml:lang="en">multilocal</skos:prefLabel>
    <skos:definition xml:lang="en">Published or produced by or for a multilocal jurisdiction which is defined as a regional combination of jurisdictions below the state level.</skos:definition>
    <skos:notation>c</skos:notation>
  </rdf:Description>
</rdf:RDF>