<?xml version="1.0" encoding="utf-8"?>
<rdf:RDF
   xmlns:dc="http://purl.org/dc/elements/1.1/"
   xmlns:dct="http://purl.org/dc/terms/"
   xmlns:rdf="http://www.w3.org/1999/02/22-rdf-syntax-ns#"
   xmlns:schema="https://schema.org/"
   xmlns:skos="http://www.w3.org/2004/02/skos/core#"
>
  <rdf:Description rdf:about="https://doi.org/10.6069/uwlswd.exen-6x37">
    <rdf:type rdf:resource="http://www.w3.org/2004/02/skos/core#ConceptScheme"/>
    <dct:type rdf:resource="http://purl.org/dc/dcmitype/Dataset"/>
    <dct:title xml:lang="en">All: place of publication production execution</dct:title>
    <dct:alternative xml:lang="en">MARC21 008/15-17 values for all materials expressed using RDF</dct:alternative>
    <dct:description xml:lang="en">Indicates the place of publication, production, or execution.</dct:description>
    <schema:disambiguatingDescription xml:lang="en">SKOS Concept Scheme for MARC 00X Values</schema:disambiguatingDescription>
    <dct:publisher rdf:resource="http://viaf.org/viaf/139541794"/>
    <dct:source rdf:resource="https://www.loc.gov/marc/bibliographic/bd008.html"/>
    <dct:source rdf:resource="http://marc21rdf.info"/>
    <dct:provenance rdf:resource="https://doi.org/10.6069/uwlswd.2e2b-y833#marc00Xvalues"/>
    <dct:creator rdf:resource="http://viaf.org/viaf/139541794"/>
    <dct:contributor rdf:resource="http://viaf.org/viaf/151962300"/>
    <dc:contributor xml:lang="en">Metadata Management Associates</dc:contributor>
    <dct:issued>2024</dct:issued>
    <dc:language>en</dc:language>
    <dct:license rdf:resource="http://creativecommons.org/publicdomain/zero/1.0"/>
    <schema:version>1-1-0</schema:version>
    <dct:format rdf:resource="http://www.w3.org/ns/formats/RDF_XML"/>
  </rdf:Description>
  <rdf:Description rdf:about="https://doi.org/10.6069/uwlswd.exen-6x37#bracketaaabracket">
    <rdf:type rdf:resource="http://www.w3.org/2004/02/skos/core#Concept"/>
    <skos:inScheme rdf:resource="https://doi.org/10.6069/uwlswd.exen-6x37"/>
    <skos:prefLabel xml:lang="en">three-character alphabetic code</skos:prefLabel>
    <skos:definition xml:lang="en">Three-character alphabetic code that indicates the place of publication, production, or execution.</skos:definition>
    <skos:scopeNote xml:lang="en">Place code is an authoritative-agency data element. Choice of a MARC code is generally related to information in field 260.</skos:scopeNote>
    <skos:notation>[aaa]</skos:notation>
  </rdf:Description>
  <rdf:Description rdf:about="https://doi.org/10.6069/uwlswd.exen-6x37#bracketaapoundbracket">
    <rdf:type rdf:resource="http://www.w3.org/2004/02/skos/core#Concept"/>
    <skos:inScheme rdf:resource="https://doi.org/10.6069/uwlswd.exen-6x37"/>
    <skos:prefLabel xml:lang="en">two-character alphabetic code</skos:prefLabel>
    <skos:definition xml:lang="en">Two-character alphabetic code that indicates the place of publication, production, or execution.</skos:definition>
    <skos:scopeNote xml:lang="en">Place code is an authoritative-agency data element. Choice of a MARC code is generally related to information in field 260.</skos:scopeNote>
    <skos:notation>[aa#]</skos:notation>
  </rdf:Description>
  <rdf:Description rdf:about="https://doi.org/10.6069/uwlswd.exen-6x37#vppound">
    <rdf:type rdf:resource="http://www.w3.org/2004/02/skos/core#Concept"/>
    <skos:inScheme rdf:resource="https://doi.org/10.6069/uwlswd.exen-6x37"/>
    <skos:prefLabel xml:lang="en">various places</skos:prefLabel>
    <skos:definition xml:lang="en">Various places are associated with different parts of items, generallly a collection.</skos:definition>
    <skos:notation>vp#</skos:notation>
  </rdf:Description>
  <rdf:Description rdf:about="https://doi.org/10.6069/uwlswd.exen-6x37#xxpound">
    <rdf:type rdf:resource="http://www.w3.org/2004/02/skos/core#Concept"/>
    <skos:inScheme rdf:resource="https://doi.org/10.6069/uwlswd.exen-6x37"/>
    <skos:prefLabel xml:lang="en">no place, unknown, or undetermined</skos:prefLabel>
    <skos:definition xml:lang="en">No place of publication, production, etc. can be provided; the place is unknown, or it is undetermined.</skos:definition>
    <skos:notation>xx#</skos:notation>
  </rdf:Description>
</rdf:RDF>
