<?xml version="1.0" encoding="utf-8"?>
<rdf:RDF
   xmlns:dc="http://purl.org/dc/elements/1.1/"
   xmlns:dct="http://purl.org/dc/terms/"
   xmlns:rdf="http://www.w3.org/1999/02/22-rdf-syntax-ns#"
   xmlns:schema="https://schema.org/"
   xmlns:skos="http://www.w3.org/2004/02/skos/core#"
>
  <rdf:Description rdf:about="https://doi.org/10.6069/uwlswd.h15g-zv41">
    <rdf:type rdf:resource="http://www.w3.org/2004/02/skos/core#ConceptScheme"/>
    <dct:type rdf:resource="http://purl.org/dc/dcmitype/Dataset"/>
    <dct:title xml:lang="en">All: modified record</dct:title>
    <dct:alternative xml:lang="en">MARC21 008/38 values for all materials expressed using RDF</dct:alternative>
    <dct:description xml:lang="en">Indicates whether any data in a bibliographic record is a modification of information that appeared on the item being cataloged or that was intended to be included in the MARC record.</dct:description>
    <schema:disambiguatingDescription xml:lang="en">SKOS Concept Scheme for MARC 00X Values</schema:disambiguatingDescription>
    <dct:publisher rdf:resource="http://viaf.org/viaf/139541794"/>
    <dct:source rdf:resource="https://www.loc.gov/marc/bibliographic/bd008.html"/>
    <dct:source rdf:resource="http://marc21rdf.info"/>
    <dct:provenance rdf:resource="https://doi.org/10.6069/uwlswd.2e2b-y833#marc00Xvalues"/>
    <dct:creator rdf:resource="http://viaf.org/viaf/139541794"/>
    <dct:contributor rdf:resource="http://viaf.org/viaf/151962300"/>
    <dc:contributor xml:lang="en">Metadata Management Associates</dc:contributor>
    <dct:issued>2024</dct:issued>
    <dc:language>en</dc:language>
    <dct:license rdf:resource="http://creativecommons.org/publicdomain/zero/1.0"/>
    <schema:version>1-1-0</schema:version>
    <dct:format rdf:resource="http://www.w3.org/ns/formats/RDF_XML"/>
  </rdf:Description>
	
  <rdf:Description rdf:about="https://doi.org/10.6069/uwlswd.h15g-zv41#pound">
    <rdf:type rdf:resource="http://www.w3.org/2004/02/skos/core#Concept"/>
    <skos:inScheme rdf:resource="https://doi.org/10.6069/uwlswd.h15g-zv41"/>
    <skos:prefLabel xml:lang="en">not modified</skos:prefLabel>
    <skos:definition xml:lang="en">Record has not been modified in any way (e.g., it is not shortened and it contains no characters that could not be converted to machine-readable form).</skos:definition>
    <skos:notation>#</skos:notation>
  </rdf:Description>
	
  <rdf:Description rdf:about="https://doi.org/10.6069/uwlswd.h15g-zv41#d">
    <rdf:type rdf:resource="http://www.w3.org/2004/02/skos/core#Concept"/>
    <skos:inScheme rdf:resource="https://doi.org/10.6069/uwlswd.h15g-zv41"/>
    <skos:prefLabel xml:lang="en">dashed-on information omitted</skos:prefLabel>
    <skos:definition xml:lang="en">MARC record does not contain "dashed-on" information found on the corresponding manual copy.</skos:definition>
	  <skos:notation>d</skos:notation>
  </rdf:Description>

  <rdf:Description rdf:about="https://doi.org/10.6069/uwlswd.h15g-zv41#o">
	<rdf:type rdf:resource="http://www.w3.org/2004/02/skos/core#Concept"/>
	<skos:inScheme rdf:resource="https://doi.org/10.6069/uwlswd.h15g-zv41"/>
	<skos:prefLabel xml:lang="en">completely romanized/printed cards romanized</skos:prefLabel>
	<skos:definition xml:lang="en">Bibliographic data in the MARC record is completely romanized and any printed cards produced are also in romanized form.</skos:definition>
	  <skos:notation>o</skos:notation>
  </rdf:Description>

  <rdf:Description rdf:about="https://doi.org/10.6069/uwlswd.h15g-zv41#r">
	<rdf:type rdf:resource="http://www.w3.org/2004/02/skos/core#Concept"/>
	<skos:inScheme rdf:resource="https://doi.org/10.6069/uwlswd.h15g-zv41"/>
	<skos:prefLabel xml:lang="en">completely romanized/printed cards in script</skos:prefLabel>
	<skos:definition xml:lang="en">Bibliographic data in the MARC record is completely romanized but the printed cards are available in the original (vernacular) script.</skos:definition>
	<skos:notation>r</skos:notation>
  </rdf:Description>

  <rdf:Description rdf:about="https://doi.org/10.6069/uwlswd.h15g-zv41#s">
	<rdf:type rdf:resource="http://www.w3.org/2004/02/skos/core#Concept"/>
	<skos:inScheme rdf:resource="https://doi.org/10.6069/uwlswd.h15g-zv41"/>
	<skos:prefLabel xml:lang="en">shortened</skos:prefLabel>
	<skos:definition xml:lang="en">Some of the data was omitted because the data exceeded the maximum length allowed by the system used to create or process it.</skos:definition>
	<skos:notation>s</skos:notation>
  </rdf:Description>

  <rdf:Description rdf:about="https://doi.org/10.6069/uwlswd.h15g-zv41#x">
	<rdf:type rdf:resource="http://www.w3.org/2004/02/skos/core#Concept"/>
	<skos:inScheme rdf:resource="https://doi.org/10.6069/uwlswd.h15g-zv41"/>
	<skos:prefLabel xml:lang="en">missing characters</skos:prefLabel>
	<skos:definition xml:lang="en">Record contained characters that could not be converted to machine_readable form (e.g., incidental nonroman characters on predominantly roman alphabet records, mathematical symbols, etc.).</skos:definition>
	<skos:notation>x</skos:notation>
  </rdf:Description>
</rdf:RDF>
