<?xml version="1.0" encoding="utf-8"?>
<rdf:RDF
   xmlns:dc="http://purl.org/dc/elements/1.1/"
   xmlns:dct="http://purl.org/dc/terms/"
   xmlns:rdf="http://www.w3.org/1999/02/22-rdf-syntax-ns#"
   xmlns:schema="https://schema.org/"
   xmlns:skos="http://www.w3.org/2004/02/skos/core#"
>
  <rdf:Description rdf:about="https://doi.org/10.6069/uwlswd.633m-h220#g">
    <rdf:type rdf:resource="http://www.w3.org/2004/02/skos/core#Concept"/>
    <skos:inScheme rdf:resource="https://doi.org/10.6069/uwlswd.633m-h220"/>
    <skos:prefLabel xml:lang="en">legal articles</skos:prefLabel>
    <skos:definition xml:lang="en">Substantive articles on legal topics, such as those published in law school reviews.</skos:definition>
    <skos:notation xml:lang="en">g</skos:notation>
  </rdf:Description>
  <rdf:Description rdf:about="https://doi.org/10.6069/uwlswd.633m-h220#q">
    <rdf:type rdf:resource="http://www.w3.org/2004/02/skos/core#Concept"/>
    <skos:inScheme rdf:resource="https://doi.org/10.6069/uwlswd.633m-h220"/>
    <skos:prefLabel xml:lang="en">filmographies</skos:prefLabel>
    <skos:definition xml:lang="en">Significant part of the item is a filmography or other bibliography of moving images.</skos:definition>
    <skos:scopeNote xml:lang="en">Used only if the filmography is substantial enough to be mentioned in the bibliographic record.</skos:scopeNote>
    <skos:notation xml:lang="en">q</skos:notation>
  </rdf:Description>
  <rdf:Description rdf:about="https://doi.org/10.6069/uwlswd.633m-h220#t">
    <rdf:type rdf:resource="http://www.w3.org/2004/02/skos/core#Concept"/>
    <skos:inScheme rdf:resource="https://doi.org/10.6069/uwlswd.633m-h220"/>
    <skos:prefLabel xml:lang="en">technical reports</skos:prefLabel>
    <skos:definition xml:lang="en">Work that is the result of scientific investigation or technical development, testing, or evaluation, presented in a form suitable for dissemination to the technical community.</skos:definition>
    <skos:notation xml:lang="en">t</skos:notation>
  </rdf:Description>
  <rdf:Description rdf:about="https://doi.org/10.6069/uwlswd.633m-h220#nx">
    <rdf:type rdf:resource="http://www.w3.org/2004/02/skos/core#Concept"/>
    <skos:inScheme rdf:resource="https://doi.org/10.6069/uwlswd.633m-h220"/>
    <skos:prefLabel xml:lang="en">legal cases and case notes [obsolete]</skos:prefLabel>
    <skos:notation xml:lang="en">n</skos:notation>
  </rdf:Description>
  <rdf:Description rdf:about="https://doi.org/10.6069/uwlswd.633m-h220#o">
    <rdf:type rdf:resource="http://www.w3.org/2004/02/skos/core#Concept"/>
    <skos:inScheme rdf:resource="https://doi.org/10.6069/uwlswd.633m-h220"/>
    <skos:prefLabel xml:lang="en">reviews</skos:prefLabel>
    <skos:definition xml:lang="en">Includes critical reviews of published or performed works (e.g., books, films, sound recordings, theater, etc.).</skos:definition>
    <skos:notation xml:lang="en">o</skos:notation>
  </rdf:Description>
  <rdf:Description rdf:about="https://doi.org/10.6069/uwlswd.633m-h220#hx">
    <rdf:type rdf:resource="http://www.w3.org/2004/02/skos/core#Concept"/>
    <skos:inScheme rdf:resource="https://doi.org/10.6069/uwlswd.633m-h220"/>
    <skos:prefLabel xml:lang="en">handbooks [obsolete]</skos:prefLabel>
    <skos:notation xml:lang="en">h</skos:notation>
  </rdf:Description>
  <rdf:Description rdf:about="https://doi.org/10.6069/uwlswd.633m-h220#m">
    <rdf:type rdf:resource="http://www.w3.org/2004/02/skos/core#Concept"/>
    <skos:inScheme rdf:resource="https://doi.org/10.6069/uwlswd.633m-h220"/>
    <skos:prefLabel xml:lang="en">theses</skos:prefLabel>
    <skos:definition xml:lang="en">Thesis, dissertation, or work identified as having been created to satisfy the requirements for an academic certification or degree.</skos:definition>
    <skos:notation xml:lang="en">m</skos:notation>
  </rdf:Description>
  <rdf:Description rdf:about="https://doi.org/10.6069/uwlswd.633m-h220#b">
    <rdf:type rdf:resource="http://www.w3.org/2004/02/skos/core#Concept"/>
    <skos:inScheme rdf:resource="https://doi.org/10.6069/uwlswd.633m-h220"/>
    <skos:prefLabel xml:lang="en">bibliographies</skos:prefLabel>
    <skos:definition xml:lang="en">Significant part of the item is a bibliography or bibliographies.</skos:definition>
    <skos:scopeNote xml:lang="en">Used only if the bibliography is substantial enough to be mentioned in the bibliographic record. Not used if also coded as a survey of literature in a subject area.</skos:scopeNote>
    <skos:notation xml:lang="en">b</skos:notation>
  </rdf:Description>
  <rdf:Description rdf:about="https://doi.org/10.6069/uwlswd.633m-h220#w">
    <rdf:type rdf:resource="http://www.w3.org/2004/02/skos/core#Concept"/>
    <skos:inScheme rdf:resource="https://doi.org/10.6069/uwlswd.633m-h220"/>
    <skos:prefLabel xml:lang="en">law reports and digests</skos:prefLabel>
    <skos:definition xml:lang="en">Texts of decisions of courts or administrative agencies.</skos:definition>
    <skos:notation xml:lang="en">w</skos:notation>
    <skos:scopeNote xml:lang="en">Also used when an item includes texts of digests of such decisions.</skos:scopeNote>
  </rdf:Description>
  <rdf:Description rdf:about="https://doi.org/10.6069/uwlswd.633m-h220">
    <rdf:type rdf:resource="http://www.w3.org/2004/02/skos/core#ConceptScheme"/>
    <dct:type rdf:resource="http://purl.org/dc/dcmitype/Dataset"/>
    <dct:title xml:lang="en">Some: nature of contents</dct:title>
    <dct:alternative xml:lang="en">MARC21 008/24-27 values for some materials expressed using RDF</dct:alternative>
    <dct:description xml:lang="en">Indicates whether a significant part of the item is or contains certain types of material.</dct:description>
    <schema:disambiguatingDescription>SKOS Concept Scheme for MARC 00X Values</schema:disambiguatingDescription>
    <dct:publisher rdf:resource="http://viaf.org/viaf/139541794"/>
    <dct:source rdf:resource="https://www.loc.gov/marc/bibliographic/bd008.html"/>
    <dct:source rdf:resource="http://marc21rdf.info"/>
    <dct:provenance rdf:resource="https://doi.org/10.6069/uwlswd.2e2b-y833"/>
    <dct:creator rdf:resource="http://viaf.org/viaf/139541794"/>
    <dct:contributor rdf:resource="http://viaf.org/viaf/151962300"/>
    <dc:contributor xml:lang="en">Metadata Management Associates</dc:contributor>
    <dct:issued>2023</dct:issued>
    <dc:language>en</dc:language>
    <dct:license rdf:resource="http://creativecommons.org/publicdomain/zero/1.0"/>
    <schema:version>1-0-1</schema:version>
    <dct:hasFormat rdf:resource="https://uwlib-cams.github.io/uwlswd_vocabs_marc_006_008/008/some_nature_of_contents/some_nature_of_contents.ttl"/>
    <dct:hasFormat rdf:resource="https://uwlib-cams.github.io/uwlswd_vocabs_marc_006_008/008/some_nature_of_contents/some_nature_of_contents.nt"/>
    <dct:hasFormat rdf:resource="https://uwlib-cams.github.io/uwlswd_vocabs_marc_006_008/008/some_nature_of_contents/some_nature_of_contents.jsonld"/>
    <dct:hasFormat rdf:resource="https://uwlib-cams.github.io/uwlswd_vocabs_marc_006_008/008/some_nature_of_contents/some_nature_of_contents.html"/>
    <dct:format rdf:resource="http://www.w3.org/ns/formats/RDF_XML"/>
  </rdf:Description>
  <rdf:Description rdf:about="https://doi.org/10.6069/uwlswd.633m-h220#y">
    <rdf:type rdf:resource="http://www.w3.org/2004/02/skos/core#Concept"/>
    <skos:inScheme rdf:resource="https://doi.org/10.6069/uwlswd.633m-h220"/>
    <skos:prefLabel xml:lang="en">yearbooks</skos:prefLabel>
    <skos:definition xml:lang="en">Reference publication issued on an annual or less frequent basis that contains articles summarizing the accomplishments or events of a particular year within a specific discipline or area of endeavor.</skos:definition>
    <skos:notation xml:lang="en">y</skos:notation>
    <skos:scopeNote xml:lang="en">Not used for annual reports, which are administrative overviews of an organization.</skos:scopeNote>
  </rdf:Description>
  <rdf:Description rdf:about="https://doi.org/10.6069/uwlswd.633m-h220#xx">
    <rdf:type rdf:resource="http://www.w3.org/2004/02/skos/core#Concept"/>
    <skos:inScheme rdf:resource="https://doi.org/10.6069/uwlswd.633m-h220"/>
    <skos:prefLabel xml:lang="en">technical reports [obsolete]</skos:prefLabel>
    <skos:notation xml:lang="en">x</skos:notation>
  </rdf:Description>
  <rdf:Description rdf:about="https://doi.org/10.6069/uwlswd.633m-h220#v">
    <rdf:type rdf:resource="http://www.w3.org/2004/02/skos/core#Concept"/>
    <skos:inScheme rdf:resource="https://doi.org/10.6069/uwlswd.633m-h220"/>
    <skos:prefLabel xml:lang="en">legal cases and case notes</skos:prefLabel>
    <skos:definition xml:lang="en">Discussions, such as those in the case comments section of law school reviews, of particular legal cases that have been decided by, or that are pending before, courts or administrative agencies.</skos:definition>
    <skos:notation xml:lang="en">v</skos:notation>
  </rdf:Description>
  <rdf:Description rdf:about="https://doi.org/10.6069/uwlswd.633m-h220#l">
    <rdf:type rdf:resource="http://www.w3.org/2004/02/skos/core#Concept"/>
    <skos:inScheme rdf:resource="https://doi.org/10.6069/uwlswd.633m-h220"/>
    <skos:prefLabel xml:lang="en">legislation</skos:prefLabel>
    <skos:definition xml:lang="en">Full or partial texts of enactments of legislative bodies, published either in statute or in code form, or texts of rules and regulations issued by executive or administrative agencies.</skos:definition>
    <skos:notation xml:lang="en">l</skos:notation>
  </rdf:Description>
  <rdf:Description rdf:about="https://doi.org/10.6069/uwlswd.633m-h220#s">
    <rdf:type rdf:resource="http://www.w3.org/2004/02/skos/core#Concept"/>
    <skos:inScheme rdf:resource="https://doi.org/10.6069/uwlswd.633m-h220"/>
    <skos:prefLabel xml:lang="en">statistics</skos:prefLabel>
    <skos:definition xml:lang="en">Significant part of the item is a collection of statistical data on a subject.</skos:definition>
    <skos:notation xml:lang="en">s</skos:notation>
    <skos:scopeNote xml:lang="en">Not used for works about statistical methodology.</skos:scopeNote>
  </rdf:Description>
  <rdf:Description rdf:about="https://doi.org/10.6069/uwlswd.633m-h220#r">
    <rdf:type rdf:resource="http://www.w3.org/2004/02/skos/core#Concept"/>
    <skos:inScheme rdf:resource="https://doi.org/10.6069/uwlswd.633m-h220"/>
    <skos:prefLabel xml:lang="en">directories</skos:prefLabel>
    <skos:definition xml:lang="en">Directory or register of persons or corporate bodies.</skos:definition>
    <skos:notation xml:lang="en">r</skos:notation>
    <skos:scopeNote xml:lang="en">Not used for serial or monographic biographical dictionaries.</skos:scopeNote>
  </rdf:Description>
  <rdf:Description rdf:about="https://doi.org/10.6069/uwlswd.633m-h220#c">
    <rdf:type rdf:resource="http://www.w3.org/2004/02/skos/core#Concept"/>
    <skos:inScheme rdf:resource="https://doi.org/10.6069/uwlswd.633m-h220"/>
    <skos:prefLabel xml:lang="en">catalogs</skos:prefLabel>
    <skos:definition xml:lang="en">List of items in a collection.</skos:definition>
    <skos:notation xml:lang="en">c</skos:notation>
    <skos:scopeNote xml:lang="en">Also includes lists of collectible objects, such as stamps and coins, or trade catalogs.</skos:scopeNote>
  </rdf:Description>
  <rdf:Description rdf:about="https://doi.org/10.6069/uwlswd.633m-h220#u">
    <rdf:type rdf:resource="http://www.w3.org/2004/02/skos/core#Concept"/>
    <skos:inScheme rdf:resource="https://doi.org/10.6069/uwlswd.633m-h220"/>
    <skos:prefLabel xml:lang="en">standards or specifications</skos:prefLabel>
    <skos:definition xml:lang="en">Either an international, national or industry standard or a specification which gives a precise statement of a process or a service requirement.</skos:definition>
    <skos:notation xml:lang="en">u</skos:notation>
  </rdf:Description>
  <rdf:Description rdf:about="https://doi.org/10.6069/uwlswd.633m-h220#5">
    <rdf:type rdf:resource="http://www.w3.org/2004/02/skos/core#Concept"/>
    <skos:inScheme rdf:resource="https://doi.org/10.6069/uwlswd.633m-h220"/>
    <skos:prefLabel xml:lang="en">calendars</skos:prefLabel>
    <skos:definition xml:lang="en">Published systems of organizing days. These may be academic calendars or almanacs, calendars published by bodies, such as labor organizations, library associations, etc.</skos:definition>
    <skos:notation xml:lang="en">5</skos:notation>
  </rdf:Description>
  <rdf:Description rdf:about="https://doi.org/10.6069/uwlswd.633m-h220#d">
    <rdf:type rdf:resource="http://www.w3.org/2004/02/skos/core#Concept"/>
    <skos:inScheme rdf:resource="https://doi.org/10.6069/uwlswd.633m-h220"/>
    <skos:prefLabel xml:lang="en">dictionaries</skos:prefLabel>
    <skos:definition xml:lang="en">Dictionaries.</skos:definition>
    <skos:notation xml:lang="en">d</skos:notation>
    <skos:scopeNote xml:lang="en">Used for a glossary or a gazetteer. Not used for concordance or serial biographical dictionaries.</skos:scopeNote>
  </rdf:Description>
  <rdf:Description rdf:about="https://doi.org/10.6069/uwlswd.633m-h220#a">
    <rdf:type rdf:resource="http://www.w3.org/2004/02/skos/core#Concept"/>
    <skos:inScheme rdf:resource="https://doi.org/10.6069/uwlswd.633m-h220"/>
    <skos:prefLabel xml:lang="en">abstracts/summaries</skos:prefLabel>
    <skos:definition xml:lang="en">Abstracts or summaries of other publications.</skos:definition>
    <skos:notation xml:lang="en">a</skos:notation>
    <skos:scopeNote xml:lang="en">Not used when a publication includes an abstract or summary of its own content.</skos:scopeNote>
  </rdf:Description>
  <rdf:Description rdf:about="https://doi.org/10.6069/uwlswd.633m-h220#n">
    <rdf:type rdf:resource="http://www.w3.org/2004/02/skos/core#Concept"/>
    <skos:inScheme rdf:resource="https://doi.org/10.6069/uwlswd.633m-h220"/>
    <skos:prefLabel xml:lang="en">surveys of literature in a subject area</skos:prefLabel>
    <skos:definition xml:lang="en">Authored surveys that summarize what has been published about a subject. Usually has a list of references either in the body of the work or as a bibliography.</skos:definition>
    <skos:notation xml:lang="en">n</skos:notation>
    <skos:scopeNote xml:lang="en">Includes authored surveys that summarize what has been published about a subject</skos:scopeNote>
  </rdf:Description>
  <rdf:Description rdf:about="https://doi.org/10.6069/uwlswd.633m-h220#h">
    <rdf:type rdf:resource="http://www.w3.org/2004/02/skos/core#Concept"/>
    <skos:inScheme rdf:resource="https://doi.org/10.6069/uwlswd.633m-h220"/>
    <skos:prefLabel xml:lang="en">biography</skos:prefLabel>
    <skos:definition xml:lang="en">Significant part of the item contains biographical material, whether autobiography, individual biography, or collective biography.</skos:definition>
    <skos:notation xml:lang="en">h</skos:notation>
    <skos:scopeNote xml:lang="en">Not used for genealogy.</skos:scopeNote>
  </rdf:Description>
  <rdf:Description rdf:about="https://doi.org/10.6069/uwlswd.633m-h220#p">
    <rdf:type rdf:resource="http://www.w3.org/2004/02/skos/core#Concept"/>
    <skos:inScheme rdf:resource="https://doi.org/10.6069/uwlswd.633m-h220"/>
    <skos:prefLabel xml:lang="en">programmed texts</skos:prefLabel>
    <skos:definition xml:lang="en">Programmed texts.</skos:definition>
    <skos:notation xml:lang="en">p</skos:notation>
  </rdf:Description>
  <rdf:Description rdf:about="https://doi.org/10.6069/uwlswd.633m-h220#6">
    <rdf:type rdf:resource="http://www.w3.org/2004/02/skos/core#Concept"/>
    <skos:inScheme rdf:resource="https://doi.org/10.6069/uwlswd.633m-h220"/>
    <skos:prefLabel xml:lang="en">comics or graphic novels</skos:prefLabel>
    <skos:definition xml:lang="en">Instances of "sequential art" in which a story (whether fact or fiction) is told primarily through a set of images (often in the form of multiple "panels" per page) presented concurrently but meant to be "read" sequentially by the viewer. The accompanying narrative and/or dialog text, when it occurs, works integrally with the images to tell the story.</skos:definition>
    <skos:notation xml:lang="en">6</skos:notation>
  </rdf:Description>
  <rdf:Description rdf:about="https://doi.org/10.6069/uwlswd.633m-h220#pound">
    <rdf:type rdf:resource="http://www.w3.org/2004/02/skos/core#Concept"/>
    <skos:inScheme rdf:resource="https://doi.org/10.6069/uwlswd.633m-h220"/>
    <skos:prefLabel xml:lang="en">no specified nature of contents</skos:prefLabel>
    <skos:definition xml:lang="en">No specified nature of contents.</skos:definition>
    <skos:notation xml:lang="en">#</skos:notation>
  </rdf:Description>
  <rdf:Description rdf:about="https://doi.org/10.6069/uwlswd.633m-h220#f">
    <rdf:type rdf:resource="http://www.w3.org/2004/02/skos/core#Concept"/>
    <skos:inScheme rdf:resource="https://doi.org/10.6069/uwlswd.633m-h220"/>
    <skos:prefLabel xml:lang="en">handbooks</skos:prefLabel>
    <skos:definition xml:lang="en">Handbooks.</skos:definition>
    <skos:notation xml:lang="en">f</skos:notation>
  </rdf:Description>
  <rdf:Description rdf:about="https://doi.org/10.6069/uwlswd.633m-h220#e">
    <rdf:type rdf:resource="http://www.w3.org/2004/02/skos/core#Concept"/>
    <skos:inScheme rdf:resource="https://doi.org/10.6069/uwlswd.633m-h220"/>
    <skos:prefLabel xml:lang="en">encyclopedias</skos:prefLabel>
    <skos:definition xml:lang="en">Encyclopedia or an encyclopedic treatment of a specific topic.</skos:definition>
    <skos:notation xml:lang="en">e</skos:notation>
  </rdf:Description>
  <rdf:Description rdf:about="https://doi.org/10.6069/uwlswd.633m-h220#i">
    <rdf:type rdf:resource="http://www.w3.org/2004/02/skos/core#Concept"/>
    <skos:inScheme rdf:resource="https://doi.org/10.6069/uwlswd.633m-h220"/>
    <skos:prefLabel xml:lang="en">indexes</skos:prefLabel>
    <skos:definition xml:lang="en">Index to bibliographical material other than itself (e.g., an indexing journal).</skos:definition>
    <skos:notation xml:lang="en">i</skos:notation>
    <skos:scopeNote xml:lang="en">Not used when a publication contains an index to its own content.</skos:scopeNote>
  </rdf:Description>
  <rdf:Description rdf:about="https://doi.org/10.6069/uwlswd.633m-h220#2">
    <rdf:type rdf:resource="http://www.w3.org/2004/02/skos/core#Concept"/>
    <skos:inScheme rdf:resource="https://doi.org/10.6069/uwlswd.633m-h220"/>
    <skos:prefLabel xml:lang="en">offprints</skos:prefLabel>
    <skos:definition xml:lang="en">Publication that originally was published as an article in a monograph or a serial and that is also issued separately and independently.</skos:definition>
    <skos:scopeNote xml:lang="en">Includes preprints and postprints.</skos:scopeNote>
    <skos:notation xml:lang="en">2</skos:notation>
  </rdf:Description>
  <rdf:Description rdf:about="https://doi.org/10.6069/uwlswd.633m-h220#k">
    <rdf:type rdf:resource="http://www.w3.org/2004/02/skos/core#Concept"/>
    <skos:inScheme rdf:resource="https://doi.org/10.6069/uwlswd.633m-h220"/>
    <skos:prefLabel xml:lang="en">discographies</skos:prefLabel>
    <skos:definition xml:lang="en">Significant part of the item is a discography or discographies, or other bibliography of recorded sound.</skos:definition>
    <skos:scopeNote xml:lang="en">Used only if the discography is substantial enough to be mentioned in the bibliographic record.</skos:scopeNote>
    <skos:notation xml:lang="en">k</skos:notation>
  </rdf:Description>
  <rdf:Description rdf:about="https://doi.org/10.6069/uwlswd.633m-h220#z">
    <rdf:type rdf:resource="http://www.w3.org/2004/02/skos/core#Concept"/>
    <skos:inScheme rdf:resource="https://doi.org/10.6069/uwlswd.633m-h220"/>
    <skos:prefLabel xml:lang="en">treaties</skos:prefLabel>
    <skos:definition xml:lang="en">Treaty or accord negotiated between two or more parties to settle a disagreement, establish a relationship, grant rights, etc.</skos:definition>
    <skos:notation xml:lang="en">z</skos:notation>
  </rdf:Description>
  <rdf:Description rdf:about="https://doi.org/10.6069/uwlswd.633m-h220#j">
    <rdf:type rdf:resource="http://www.w3.org/2004/02/skos/core#Concept"/>
    <skos:inScheme rdf:resource="https://doi.org/10.6069/uwlswd.633m-h220"/>
    <skos:prefLabel xml:lang="en">patent document</skos:prefLabel>
    <skos:definition xml:lang="en">Detailed description of an invention or discovery of a new and useful process, machine, manufacture, composition of matter, or improvements thereof.</skos:definition>
    <skos:notation xml:lang="en">j</skos:notation>
    <skos:scopeNote xml:lang="en">A patent document may be one of several kinds of documents: a patent or similar document (e.g., inventor's certificate), a patent application (domestic, foreign, priority application, etc.), or a continuation/division of one of the above.</skos:scopeNote>
  </rdf:Description>
</rdf:RDF>
