<?xml version='1.0' encoding='UTF-8'?>
<rdf:RDF xmlns:dc="http://purl.org/dc/elements/1.1/" xmlns:dct="http://purl.org/dc/terms/" xmlns:rdf="http://www.w3.org/1999/02/22-rdf-syntax-ns#" xmlns:schema="https://schema.org/" xmlns:skos="http://www.w3.org/2004/02/skos/core#">
  <rdf:Description rdf:about="https://doi.org/10.6069/uwlswd.npns-e903#u">
    <rdf:type rdf:resource="http://www.w3.org/2004/02/skos/core#Concept"/>
    <skos:inScheme rdf:resource="https://doi.org/10.6069/uwlswd.npns-e903"/>
    <skos:prefLabel xml:lang="en">unknown</skos:prefLabel>
    <skos:definition xml:lang="en">Regularity of the item is unknown.</skos:definition>
    <skos:notation>u</skos:notation>
  </rdf:Description>
  <rdf:Description rdf:about="https://doi.org/10.6069/uwlswd.npns-e903#r">
    <rdf:type rdf:resource="http://www.w3.org/2004/02/skos/core#Concept"/>
    <skos:inScheme rdf:resource="https://doi.org/10.6069/uwlswd.npns-e903"/>
    <skos:prefLabel xml:lang="en">regular</skos:prefLabel>
    <skos:definition xml:lang="en">Intended regular publishing pattern.</skos:definition>
    <skos:scopeNote xml:lang="en">This may be determined from information on the piece or by examining the publishing pattern. Thus, use this pattern if an item states that it is to be issued, for example, bimonthly, even though the publishing pattern is known to have occasional variations due to publishing difficulties.</skos:scopeNote>
    <skos:notation>r</skos:notation>
  </rdf:Description>
  <rdf:Description rdf:about="https://doi.org/10.6069/uwlswd.npns-e903#x">
    <rdf:type rdf:resource="http://www.w3.org/2004/02/skos/core#Concept"/>
    <skos:inScheme rdf:resource="https://doi.org/10.6069/uwlswd.npns-e903"/>
    <skos:prefLabel xml:lang="en">completely irregular</skos:prefLabel>
    <skos:definition xml:lang="en">Intentionally irregular.</skos:definition>
    <skos:scopeNote xml:lang="en">Used when the frequency is known to be intentionally irregular.</skos:scopeNote>
    <skos:notation>x</skos:notation>
  </rdf:Description>
  <rdf:Description rdf:about="https://doi.org/10.6069/uwlswd.npns-e903">
    <rdf:type rdf:resource="http://www.w3.org/2004/02/skos/core#ConceptScheme"/>
    <dct:type rdf:resource="http://purl.org/dc/dcmitype/Dataset"/>
    <dct:title xml:lang="en">Continuing: regularity</dct:title>
    <dct:alternative xml:lang="en">MARC21 008/19 values for continuing resources expressed using RDF</dct:alternative>
    <dct:description xml:lang="en">Indicates the intended regularity of an item.</dct:description>
    <schema:disambiguatingDescription xml:lang="en">SKOS Concept Scheme for MARC 00X Values</schema:disambiguatingDescription>
    <dct:publisher rdf:resource="http://viaf.org/viaf/139541794"/>
    <dct:source rdf:resource="https://www.loc.gov/marc/bibliographic/bd008.html"/>
    <dct:source rdf:resource="http://marc21rdf.info"/>
    <dct:provenance rdf:resource="https://doi.org/10.6069/uwlswd.2e2b-y833#marc00Xvalues"/>
    <dct:creator rdf:resource="http://viaf.org/viaf/139541794"/>
    <dct:contributor rdf:resource="http://viaf.org/viaf/151962300"/>
    <dc:contributor xml:lang="en">Metadata Management Associates</dc:contributor>
    <dct:issued>2023</dct:issued>
    <dc:language>en</dc:language>
    <dct:license rdf:resource="http://creativecommons.org/publicdomain/zero/1.0"/>
    <schema:version>1-0-1</schema:version>
    <dct:hasFormat rdf:resource="https://uwlib-cams.github.io/uwlswd_vocabs_marc_006_008/008/continuing_regularity/continuing_regularity.ttl"/>
    <dct:hasFormat rdf:resource="https://uwlib-cams.github.io/uwlswd_vocabs_marc_006_008/008/continuing_regularity/continuing_regularity.nt"/>
    <dct:hasFormat rdf:resource="https://uwlib-cams.github.io/uwlswd_vocabs_marc_006_008/008/continuing_regularity/continuing_regularity.jsonld"/>
    <dct:hasFormat rdf:resource="https://uwlib-cams.github.io/uwlswd_vocabs_marc_006_008/008/continuing_regularity/continuing_regularity.html"/>
    <dct:format rdf:resource="http://www.w3.org/ns/formats/RDF_XML"/>
  </rdf:Description>
  <rdf:Description rdf:about="https://doi.org/10.6069/uwlswd.npns-e903#n">
    <rdf:type rdf:resource="http://www.w3.org/2004/02/skos/core#Concept"/>
    <skos:inScheme rdf:resource="https://doi.org/10.6069/uwlswd.npns-e903"/>
    <skos:prefLabel xml:lang="en">normalized irregular</skos:prefLabel>
    <skos:definition xml:lang="en">Predictable irregularity pattern.</skos:definition>
    <skos:scopeNote xml:lang="en">Used, for example, when the publishing pattern intentionally deviates from a standard pattern (example: Monthly, except July and Aug) or to accommodate an annual cumulation.</skos:scopeNote>
    <skos:notation>n</skos:notation>
  </rdf:Description>
</rdf:RDF>