@prefix dc: <http://purl.org/dc/elements/1.1/> .
@prefix dct: <http://purl.org/dc/terms/> .
@prefix schema: <https://schema.org/> .
@prefix skos: <http://www.w3.org/2004/02/skos/core#> .

<https://doi.org/10.6069/uwlswd.b5wb-fr38#bracketaaabracket> a skos:Concept ;
    skos:definition "Three-character alphabetic code that indicates the language of the item. Choice of a MARC code is based on the predominant language of the item."@en ;
    skos:inScheme <https://doi.org/10.6069/uwlswd.b5wb-fr38> ;
    skos:notation "[aaa]" ;
    skos:prefLabel "three-character alphabetic code"@en .

<https://doi.org/10.6069/uwlswd.b5wb-fr38#mul> a skos:Concept ;
    skos:definition "Item is multilingual with no predominant language and the cataloging institution has chosen not to specify a language in 008/35-37."@en ;
    skos:inScheme <https://doi.org/10.6069/uwlswd.b5wb-fr38> ;
    skos:notation "mul" ;
    skos:prefLabel "multiple languages"@en .

<https://doi.org/10.6069/uwlswd.b5wb-fr38#poundpoundpound> a skos:Concept ;
    skos:definition "No information provided."@en ;
    skos:inScheme <https://doi.org/10.6069/uwlswd.b5wb-fr38> ;
    skos:notation "###" ;
    skos:prefLabel "no information provided"@en .

<https://doi.org/10.6069/uwlswd.b5wb-fr38#sgn> a skos:Concept ;
    skos:definition "Primary medium of communication is a sign language."@en ;
    skos:inScheme <https://doi.org/10.6069/uwlswd.b5wb-fr38> ;
    skos:notation "sgn" ;
    skos:prefLabel "sign languages"@en ;
    skos:scopeNote "E.g., a book containing pictures of the handshape of each letter of a particular sign system, or a videorecording that is signed. The particular sign language system is stated in field 546 (Language Note), e.g., American Sign Language. The codes for secondary and related languages may be indicated in field 041 (Language Code)."@en .

<https://doi.org/10.6069/uwlswd.b5wb-fr38#und> a skos:Concept ;
    skos:definition "Language of the item cannot be determined."@en ;
    skos:inScheme <https://doi.org/10.6069/uwlswd.b5wb-fr38> ;
    skos:notation "und" ;
    skos:prefLabel "undetermined"@en ;
    skos:scopeNote "Also used for works having content consisting of arbitrary syllables, humming, or other human-produced sounds for which a language cannot be specified."@en .

<https://doi.org/10.6069/uwlswd.b5wb-fr38#zxx> a skos:Concept ;
    skos:definition "Item has no sung, spoken, or written textual content."@en ;
    skos:inScheme <https://doi.org/10.6069/uwlswd.b5wb-fr38> ;
    skos:notation "zxx" ;
    skos:prefLabel "no linguistic content"@en ;
    skos:scopeNote "Examples of such items are: 1) instrumental or electronic music; 2) sound recordings consisting of nonverbal sounds; 3) moving image materials with no sound or sign language content, or if sound, no narration; 4) visual materials other than moving images with no printed titles, captions, etc.; 5) computer files that consist of no more than the machine language (e.g., COBOL) or character codes (e.g., ASCII) used in source programs."@en .

<https://doi.org/10.6069/uwlswd.b5wb-fr38> a skos:ConceptScheme ;
    dc:contributor "Metadata Management Associates"@en ;
    dc:language "en" ;
    dct:alternative "MARC21 008/35-37 values for all materials expressed using RDF"@en ;
    dct:contributor <http://viaf.org/viaf/151962300> ;
    dct:creator <http://viaf.org/viaf/139541794> ;
    dct:description "Indicates the language of the item."@en ;
    dct:format <http://www.w3.org/ns/formats/Turtle> ;
    dct:hasFormat <https://uwlib-cams.github.io/uwlswd_vocabs_marc_006_008/008/all_language/all_language.html>,
        <https://uwlib-cams.github.io/uwlswd_vocabs_marc_006_008/008/all_language/all_language.jsonld>,
        <https://uwlib-cams.github.io/uwlswd_vocabs_marc_006_008/008/all_language/all_language.nt>,
        <https://uwlib-cams.github.io/uwlswd_vocabs_marc_006_008/008/all_language/all_language.rdf> ;
    dct:issued "2024" ;
    dct:license <http://creativecommons.org/publicdomain/zero/1.0> ;
    dct:provenance <https://doi.org/10.6069/uwlswd.2e2b-y833#marc00Xvalues> ;
    dct:publisher <http://viaf.org/viaf/139541794> ;
    dct:source <http://marc21rdf.info>,
        <https://www.loc.gov/marc/bibliographic/bd008.html> ;
    dct:title "All: language"@en ;
    dct:type <http://purl.org/dc/dcmitype/Dataset> ;
    schema:disambiguatingDescription "SKOS Concept Scheme for MARC 00X Values"@en ;
    schema:version "1-1-0" .

