@prefix dc: <http://purl.org/dc/elements/1.1/> .
@prefix dct: <http://purl.org/dc/terms/> .
@prefix schema: <https://schema.org/> .
@prefix skos: <http://www.w3.org/2004/02/skos/core#> .

<https://doi.org/10.6069/uwlswd.tsh7-5175#c> a skos:Concept ;
    skos:definition "Creator of the cataloging data is a participant (other than a national bibliographic agency) in a cooperative cataloging program."@en ;
    skos:inScheme <https://doi.org/10.6069/uwlswd.tsh7-5175> ;
    skos:notation "c" ;
    skos:prefLabel "cooperative cataloging program"@en .

<https://doi.org/10.6069/uwlswd.tsh7-5175#d> a skos:Concept ;
    skos:definition "Source of the cataloging data is an organization that is other than a national bibliographic agency or a participant in a cooperative cataloging program."@en ;
    skos:inScheme <https://doi.org/10.6069/uwlswd.tsh7-5175> ;
    skos:notation "d" ;
    skos:prefLabel "other"@en .

<https://doi.org/10.6069/uwlswd.tsh7-5175#pound> a skos:Concept ;
    skos:definition "Creator of the original cataloging data is a national bibliographic agency (e.g., U.S. Library of Congress or Library and Archives Canada)."@en ;
    skos:inScheme <https://doi.org/10.6069/uwlswd.tsh7-5175> ;
    skos:notation "#" ;
    skos:prefLabel "national bibliographic agency"@en .

<https://doi.org/10.6069/uwlswd.tsh7-5175#u> a skos:Concept ;
    skos:definition "Creator of the cataloging data is unknown."@en ;
    skos:inScheme <https://doi.org/10.6069/uwlswd.tsh7-5175> ;
    skos:notation "u" ;
    skos:prefLabel "unknown"@en ;
    skos:scopeNote "Used when an organization transcribes manual cataloging data from an unknown source. In this case, field 040 lacks a subfield $a and subfield $c contains the MARC code for the transcribing organization."@en .

<https://doi.org/10.6069/uwlswd.tsh7-5175> a skos:ConceptScheme ;
    dc:contributor "Metadata Management Associates"@en ;
    dc:language "en" ;
    dct:alternative "MARC21 008/39 values for all materials expressed using RDF"@en ;
    dct:contributor <http://viaf.org/viaf/151962300> ;
    dct:creator <http://viaf.org/viaf/139541794> ;
    dct:description "Indicates the original cataloging source of the record."@en ;
    dct:format <http://www.w3.org/ns/formats/Turtle> ;
    dct:hasFormat <https://uwlib-cams.github.io/uwlswd_vocabs_marc_006_008/008/all_cataloging_source/all_cataloging_source.html>,
        <https://uwlib-cams.github.io/uwlswd_vocabs_marc_006_008/008/all_cataloging_source/all_cataloging_source.jsonld>,
        <https://uwlib-cams.github.io/uwlswd_vocabs_marc_006_008/008/all_cataloging_source/all_cataloging_source.nt>,
        <https://uwlib-cams.github.io/uwlswd_vocabs_marc_006_008/008/all_cataloging_source/all_cataloging_source.rdf> ;
    dct:issued "2024" ;
    dct:license <http://creativecommons.org/publicdomain/zero/1.0> ;
    dct:provenance <https://doi.org/10.6069/uwlswd.2e2b-y833#marc00Xvalues> ;
    dct:publisher <http://viaf.org/viaf/139541794> ;
    dct:source <http://marc21rdf.info>,
        <https://www.loc.gov/marc/bibliographic/bd008.html> ;
    dct:title "All: cataloging source"@en ;
    dct:type <http://purl.org/dc/dcmitype/Dataset> ;
    schema:disambiguatingDescription "SKOS Concept Scheme for MARC 00X Values"@en ;
    schema:version "1-1-0" .

